Reviewed/commented full_ltlTheory

examples/temporal_deep/src/deep_embeddings/full_ltlScript.sml
@@ -1,3 +1,9 @@
+(* -*- Mode: holscript; -*- ***************************************************)
+(*                                                                            *)
+(*       Linear Temporal Logic (with both past and future operators           *)
+(*                                                                            *)
+(******************************************************************************)
+
 open HolKernel Parse boolLib bossLib;
 
 open pred_setTheory prop_logicTheory xprop_logicTheory infinite_pathTheory
@@ -16,7 +22,7 @@ val _ = ParseExtras.temp_loose_equality()
 (* Syntax                                                                    *)
 (*****************************************************************************)
 
-val _ = Datatype `
+Datatype :
   ltl = LTL_PROP    ('prop prop_logic)
       | LTL_NOT      ltl
       | LTL_AND     (ltl # ltl)
@@ -24,9 +30,7 @@ val _ = Datatype `
       | LTL_SUNTIL  (ltl # ltl)  (* U in NuSMV *)
       | LTL_PSNEXT   ltl         (* Y in NuSMV *)
       | LTL_PSUNTIL (ltl # ltl)  (* S in NuSMV *)
-`;
-
-val _ = overload_on ("LTL_P_PROP", ``\p. LTL_PROP (P_PROP p)``);
+End
 
 Theorem ltl_induct = Q.GEN `P`
    (MATCH_MP
@@ -145,99 +149,103 @@ val LTL_INIT_def = Define
 ******************************************************************************)
 
 val IS_FUTURE_LTL_def = Define
-   `(IS_FUTURE_LTL (LTL_PROP b) = T) /\
-    (IS_FUTURE_LTL (LTL_NOT f) = (IS_FUTURE_LTL f)) /\
-    (IS_FUTURE_LTL (LTL_AND(f1,f2)) = (IS_FUTURE_LTL f1 /\ IS_FUTURE_LTL f2)) /\
-    (IS_FUTURE_LTL (LTL_NEXT f) = (IS_FUTURE_LTL f)) /\
-    (IS_FUTURE_LTL (LTL_SUNTIL(f1,f2)) = (IS_FUTURE_LTL f1 /\ IS_FUTURE_LTL f2)) /\
-    (IS_FUTURE_LTL (LTL_PSNEXT f) = F) /\
-    (IS_FUTURE_LTL (LTL_PSUNTIL(f1,f2)) = F)`;
+  `(IS_FUTURE_LTL (LTL_PROP b) = T) /\
+   (IS_FUTURE_LTL (LTL_NOT f) = (IS_FUTURE_LTL f)) /\
+   (IS_FUTURE_LTL (LTL_AND(f1,f2)) = (IS_FUTURE_LTL f1 /\ IS_FUTURE_LTL f2)) /\
+   (IS_FUTURE_LTL (LTL_NEXT f) = (IS_FUTURE_LTL f)) /\
+   (IS_FUTURE_LTL (LTL_SUNTIL(f1,f2)) = (IS_FUTURE_LTL f1 /\ IS_FUTURE_LTL f2)) /\
+   (IS_FUTURE_LTL (LTL_PSNEXT f) = F) /\
+   (IS_FUTURE_LTL (LTL_PSUNTIL(f1,f2)) = F)`;
 
 val IS_PAST_LTL_def = Define
-   `(IS_PAST_LTL (LTL_PROP b) = T) /\
-    (IS_PAST_LTL (LTL_NOT f) = (IS_PAST_LTL f)) /\
-    (IS_PAST_LTL (LTL_AND(f1,f2)) = (IS_PAST_LTL f1 /\ IS_PAST_LTL f2)) /\
-    (IS_PAST_LTL (LTL_PSNEXT f) = (IS_PAST_LTL f)) /\
-    (IS_PAST_LTL (LTL_PSUNTIL(f1,f2)) = (IS_PAST_LTL f1 /\ IS_PAST_LTL f2)) /\
-    (IS_PAST_LTL (LTL_NEXT f) = F) /\
-    (IS_PAST_LTL (LTL_SUNTIL(f1,f2)) = F)`;
+  `(IS_PAST_LTL (LTL_PROP b) = T) /\
+   (IS_PAST_LTL (LTL_NOT f) = (IS_PAST_LTL f)) /\
+   (IS_PAST_LTL (LTL_AND(f1,f2)) = (IS_PAST_LTL f1 /\ IS_PAST_LTL f2)) /\
+   (IS_PAST_LTL (LTL_PSNEXT f) = (IS_PAST_LTL f)) /\
+   (IS_PAST_LTL (LTL_PSUNTIL(f1,f2)) = (IS_PAST_LTL f1 /\ IS_PAST_LTL f2)) /\
+   (IS_PAST_LTL (LTL_NEXT f) = F) /\
+   (IS_PAST_LTL (LTL_SUNTIL(f1,f2)) = F)`;
 
 val IS_LTL_G_def = Define
-   `(IS_LTL_G (LTL_PROP p) = T) /\
-    (IS_LTL_G (LTL_NOT f) = IS_LTL_F f) /\
-    (IS_LTL_G (LTL_AND (f,g)) = (IS_LTL_G f /\ IS_LTL_G g)) /\
-    (IS_LTL_G (LTL_NEXT f) = IS_LTL_G f) /\
-    (IS_LTL_G (LTL_SUNTIL(f,g)) = F) /\
-    (IS_LTL_G (LTL_PSNEXT f) = IS_LTL_G f) /\
-    (IS_LTL_G (LTL_PSUNTIL(f,g)) = (IS_LTL_G f /\ IS_LTL_G g)) /\
+  `(IS_LTL_G (LTL_PROP p) = T) /\
+   (IS_LTL_G (LTL_NOT f) = IS_LTL_F f) /\
+   (IS_LTL_G (LTL_AND (f,g)) = (IS_LTL_G f /\ IS_LTL_G g)) /\
+   (IS_LTL_G (LTL_NEXT f) = IS_LTL_G f) /\
+   (IS_LTL_G (LTL_SUNTIL(f,g)) = F) /\
+   (IS_LTL_G (LTL_PSNEXT f) = IS_LTL_G f) /\
+   (IS_LTL_G (LTL_PSUNTIL(f,g)) = (IS_LTL_G f /\ IS_LTL_G g)) /\
 
-    (IS_LTL_F (LTL_PROP p) = T) /\
-    (IS_LTL_F (LTL_NOT f) = IS_LTL_G f) /\
-    (IS_LTL_F (LTL_AND (f,g)) = (IS_LTL_F f /\ IS_LTL_F g)) /\
-    (IS_LTL_F (LTL_NEXT f) = IS_LTL_F f) /\
-    (IS_LTL_F (LTL_SUNTIL(f,g)) = (IS_LTL_F f /\ IS_LTL_F g)) /\
-    (IS_LTL_F (LTL_PSNEXT f) = IS_LTL_F f) /\
-    (IS_LTL_F (LTL_PSUNTIL(f,g)) = (IS_LTL_F f /\ IS_LTL_F g))`;
+   (IS_LTL_F (LTL_PROP p) = T) /\
+   (IS_LTL_F (LTL_NOT f) = IS_LTL_G f) /\
+   (IS_LTL_F (LTL_AND (f,g)) = (IS_LTL_F f /\ IS_LTL_F g)) /\
+   (IS_LTL_F (LTL_NEXT f) = IS_LTL_F f) /\
+   (IS_LTL_F (LTL_SUNTIL(f,g)) = (IS_LTL_F f /\ IS_LTL_F g)) /\
+   (IS_LTL_F (LTL_PSNEXT f) = IS_LTL_F f) /\
+   (IS_LTL_F (LTL_PSUNTIL(f,g)) = (IS_LTL_F f /\ IS_LTL_F g))`;
 
+(* (co)safety properties *)
 val IS_LTL_PREFIX_def = Define
-   `(IS_LTL_PREFIX (LTL_NOT f) = IS_LTL_PREFIX f) /\
-    (IS_LTL_PREFIX (LTL_AND (f,g)) = (IS_LTL_PREFIX f /\ IS_LTL_PREFIX g)) /\
-    (IS_LTL_PREFIX f = (IS_LTL_G f \/ IS_LTL_F f))`;
-
+  `(IS_LTL_PREFIX (LTL_NOT f) = IS_LTL_PREFIX f) /\
+   (IS_LTL_PREFIX (LTL_AND (f,g)) = (IS_LTL_PREFIX f /\ IS_LTL_PREFIX g)) /\
+   (IS_LTL_PREFIX f = (IS_LTL_G f \/ IS_LTL_F f))`;
 
 val IS_LTL_GF_def = Define
-   `(IS_LTL_GF (LTL_PROP p) = T) /\
-    (IS_LTL_GF (LTL_NOT f) = IS_LTL_FG f) /\
-    (IS_LTL_GF (LTL_AND (f,g)) = (IS_LTL_GF f /\ IS_LTL_GF g)) /\
-    (IS_LTL_GF (LTL_NEXT f) = IS_LTL_GF f) /\
-    (IS_LTL_GF (LTL_SUNTIL(f,g)) = (IS_LTL_GF f /\ IS_LTL_F g)) /\
-    (IS_LTL_GF (LTL_PSNEXT f) = IS_LTL_GF f) /\
-    (IS_LTL_GF (LTL_PSUNTIL(f,g)) = (IS_LTL_GF f /\ IS_LTL_GF g)) /\
+  `(IS_LTL_GF (LTL_PROP p) = T) /\
+   (IS_LTL_GF (LTL_NOT f) = IS_LTL_FG f) /\
+   (IS_LTL_GF (LTL_AND (f,g)) = (IS_LTL_GF f /\ IS_LTL_GF g)) /\
+   (IS_LTL_GF (LTL_NEXT f) = IS_LTL_GF f) /\
+   (IS_LTL_GF (LTL_SUNTIL(f,g)) = (IS_LTL_GF f /\ IS_LTL_F g)) /\
+   (IS_LTL_GF (LTL_PSNEXT f) = IS_LTL_GF f) /\
+   (IS_LTL_GF (LTL_PSUNTIL(f,g)) = (IS_LTL_GF f /\ IS_LTL_GF g)) /\
 
-    (IS_LTL_FG (LTL_PROP p) = T) /\
-    (IS_LTL_FG (LTL_NOT f) = IS_LTL_GF f) /\
-    (IS_LTL_FG (LTL_AND (f,g)) = (IS_LTL_FG f /\ IS_LTL_FG g)) /\
-    (IS_LTL_FG (LTL_NEXT f) = IS_LTL_FG f) /\
-    (IS_LTL_FG (LTL_SUNTIL(f,g)) = (IS_LTL_FG f /\ IS_LTL_FG g)) /\
-    (IS_LTL_FG (LTL_PSNEXT f) = IS_LTL_FG f) /\
-    (IS_LTL_FG (LTL_PSUNTIL(f,g)) = (IS_LTL_FG f /\ IS_LTL_FG g))`;
+   (IS_LTL_FG (LTL_PROP p) = T) /\
+   (IS_LTL_FG (LTL_NOT f) = IS_LTL_GF f) /\
+   (IS_LTL_FG (LTL_AND (f,g)) = (IS_LTL_FG f /\ IS_LTL_FG g)) /\
+   (IS_LTL_FG (LTL_NEXT f) = IS_LTL_FG f) /\
+   (IS_LTL_FG (LTL_SUNTIL(f,g)) = (IS_LTL_FG f /\ IS_LTL_FG g)) /\
+   (IS_LTL_FG (LTL_PSNEXT f) = IS_LTL_FG f) /\
+   (IS_LTL_FG (LTL_PSUNTIL(f,g)) = (IS_LTL_FG f /\ IS_LTL_FG g))`;
 
 val IS_LTL_STREET_def = Define
-   `(IS_LTL_STREET (LTL_NOT f) = IS_LTL_STREET f) /\
-    (IS_LTL_STREET (LTL_AND (f,g)) = (IS_LTL_STREET f /\ IS_LTL_STREET g)) /\
-    (IS_LTL_STREET f = (IS_LTL_GF f \/ IS_LTL_FG f))`;
+  `(IS_LTL_STREET (LTL_NOT f) = IS_LTL_STREET f) /\
+   (IS_LTL_STREET (LTL_AND (f,g)) = (IS_LTL_STREET f /\ IS_LTL_STREET g)) /\
+   (IS_LTL_STREET f = (IS_LTL_GF f \/ IS_LTL_FG f))`;
 
-Theorem IS_LTL_THM =
-   LIST_CONJ [IS_FUTURE_LTL_def,
-              IS_PAST_LTL_def,
-              IS_LTL_G_def,
-              IS_LTL_GF_def,
-              IS_LTL_PREFIX_def,
-              IS_LTL_STREET_def];
+Theorem IS_LTL_THM = LIST_CONJ
+   [IS_FUTURE_LTL_def,
+    IS_PAST_LTL_def,
+    IS_LTL_G_def,
+    IS_LTL_GF_def,
+    IS_LTL_PREFIX_def,
+    IS_LTL_STREET_def];
 
 Theorem IS_LTL_RELATIONS :
-    !f. ((IS_LTL_F f = IS_LTL_G (LTL_NOT f)) /\ (IS_LTL_G f = IS_LTL_F (LTL_NOT f)) /\
-          (IS_LTL_FG f = IS_LTL_GF (LTL_NOT f)) /\ (IS_LTL_GF f = IS_LTL_FG (LTL_NOT f)) /\
-          (IS_LTL_F f ==> IS_LTL_FG f) /\ (IS_LTL_G f ==> IS_LTL_GF f) /\
-          (IS_LTL_G f ==> IS_LTL_FG f) /\ (IS_LTL_F f ==> IS_LTL_GF f) /\
-          (IS_LTL_PREFIX f ==> (IS_LTL_FG f /\ IS_LTL_GF f)))
+    !f. (IS_LTL_F f = IS_LTL_G (LTL_NOT f)) /\
+        (IS_LTL_G f = IS_LTL_F (LTL_NOT f)) /\
+        (IS_LTL_FG f = IS_LTL_GF (LTL_NOT f)) /\
+        (IS_LTL_GF f = IS_LTL_FG (LTL_NOT f)) /\
+        (IS_LTL_F f ==> IS_LTL_FG f) /\
+        (IS_LTL_G f ==> IS_LTL_GF f) /\
+        (IS_LTL_G f ==> IS_LTL_FG f) /\
+        (IS_LTL_F f ==> IS_LTL_GF f) /\
+        (IS_LTL_PREFIX f ==> IS_LTL_FG f /\ IS_LTL_GF f)
 Proof
-      INDUCT_THEN ltl_induct ASSUME_TAC THEN
-      REWRITE_TAC[IS_LTL_THM] THEN
-      METIS_TAC[]
+    INDUCT_THEN ltl_induct ASSUME_TAC
+ >> REWRITE_TAC [IS_LTL_THM]
+ >> METIS_TAC []
 QED
 
 (******************************************************************************
 * Lemmata
 ******************************************************************************)
 val LTL_USED_VARS_def = Define
-   `(LTL_USED_VARS (LTL_PROP p) = P_USED_VARS p) /\
-    (LTL_USED_VARS (LTL_NOT f) = LTL_USED_VARS f) /\
-    (LTL_USED_VARS (LTL_AND (f,g)) = (LTL_USED_VARS f UNION LTL_USED_VARS g)) /\
-    (LTL_USED_VARS (LTL_NEXT f) = LTL_USED_VARS f) /\
-    (LTL_USED_VARS (LTL_SUNTIL(f,g)) = (LTL_USED_VARS f UNION LTL_USED_VARS g)) /\
-    (LTL_USED_VARS (LTL_PSNEXT f) = LTL_USED_VARS f) /\
-    (LTL_USED_VARS (LTL_PSUNTIL(f,g)) = (LTL_USED_VARS f UNION LTL_USED_VARS g))`;
+  `(LTL_USED_VARS (LTL_PROP p) = P_USED_VARS p) /\
+   (LTL_USED_VARS (LTL_NOT f) = LTL_USED_VARS f) /\
+   (LTL_USED_VARS (LTL_AND (f,g)) = (LTL_USED_VARS f UNION LTL_USED_VARS g)) /\
+   (LTL_USED_VARS (LTL_NEXT f) = LTL_USED_VARS f) /\
+   (LTL_USED_VARS (LTL_SUNTIL(f,g)) = (LTL_USED_VARS f UNION LTL_USED_VARS g)) /\
+   (LTL_USED_VARS (LTL_PSNEXT f) = LTL_USED_VARS f) /\
+   (LTL_USED_VARS (LTL_PSUNTIL(f,g)) = (LTL_USED_VARS f UNION LTL_USED_VARS g))`;
 
 Theorem LTL_USED_VARS_INTER_SUBSET_THM :
     !f t v S. (LTL_USED_VARS f) SUBSET S ==>
@@ -246,117 +254,105 @@ Proof
    INDUCT_THEN ltl_induct ASSUME_TAC THENL [
       SIMP_TAC arith_ss [LTL_SEM_TIME_def, LTL_USED_VARS_def, PATH_RESTRICT_def, PATH_MAP_def] THEN
       PROVE_TAC[P_USED_VARS_INTER_SUBSET_THM],
-
       REWRITE_TAC[LTL_SEM_TIME_def, LTL_USED_VARS_def] THEN
       PROVE_TAC[],
-
       REWRITE_TAC[LTL_SEM_TIME_def, LTL_USED_VARS_def, UNION_SUBSET] THEN
       PROVE_TAC[],
-
       REWRITE_TAC[LTL_SEM_TIME_def, LTL_USED_VARS_def] THEN
       PROVE_TAC[],
-
       REWRITE_TAC[LTL_SEM_TIME_def, LTL_USED_VARS_def, UNION_SUBSET] THEN
       PROVE_TAC[],
-
       REWRITE_TAC[LTL_SEM_TIME_def, LTL_USED_VARS_def] THEN
       PROVE_TAC[],
-
       REWRITE_TAC[LTL_SEM_TIME_def, LTL_USED_VARS_def, UNION_SUBSET] THEN
       PROVE_TAC[]
    ]
 QED
 
-val LTL_USED_VARS_INTER_THM =
- store_thm
-  ("LTL_USED_VARS_INTER_THM",
-   ``!f t v. (LTL_SEM_TIME t v f = LTL_SEM_TIME t (PATH_RESTRICT v (LTL_USED_VARS f)) f)``,
+Theorem LTL_USED_VARS_INTER_THM :
+    !f t v. (LTL_SEM_TIME t v f = LTL_SEM_TIME t (PATH_RESTRICT v (LTL_USED_VARS f)) f)
+Proof
+    METIS_TAC [LTL_USED_VARS_INTER_SUBSET_THM, SUBSET_REFL]
+QED
 
-   METIS_TAC  [LTL_USED_VARS_INTER_SUBSET_THM, SUBSET_REFL]);
+Theorem FINITE___LTL_USED_VARS :
+    !l. FINITE (LTL_USED_VARS l)
+Proof
+    INDUCT_THEN ltl_induct ASSUME_TAC
+ >- REWRITE_TAC [LTL_USED_VARS_def, FINITE___P_USED_VARS]
+ >> ASM_REWRITE_TAC [LTL_USED_VARS_def, FINITE_UNION]
+QED
 
-val FINITE___LTL_USED_VARS =
- store_thm
-  ("FINITE___LTL_USED_VARS",
+Theorem LTL_USED_VARS_EVAL :
+    (LTL_USED_VARS (LTL_PROP p) = P_USED_VARS p) /\
+    (LTL_USED_VARS (LTL_NOT r) = LTL_USED_VARS r) /\
+    (LTL_USED_VARS (LTL_AND (r1,r2)) = LTL_USED_VARS r1 UNION LTL_USED_VARS r2) /\
+    (LTL_USED_VARS (LTL_NEXT r) = LTL_USED_VARS r) /\
+    (LTL_USED_VARS (LTL_SUNTIL(r1,r2)) = LTL_USED_VARS r1 UNION LTL_USED_VARS r2) /\
+    (LTL_USED_VARS (LTL_PSNEXT r) = LTL_USED_VARS r) /\
+    (LTL_USED_VARS (LTL_PSUNTIL(r1,r2)) = LTL_USED_VARS r1 UNION LTL_USED_VARS r2) /\
+    (LTL_USED_VARS (LTL_OR (r1,r2)) = LTL_USED_VARS r1 UNION LTL_USED_VARS r2) /\
+    (LTL_USED_VARS (LTL_IMPL (r1,r2)) = LTL_USED_VARS r1 UNION LTL_USED_VARS r2) /\
+    (LTL_USED_VARS (LTL_EQUIV (r1,r2)) = LTL_USED_VARS r1 UNION LTL_USED_VARS r2) /\
+    (LTL_USED_VARS (LTL_ALWAYS r) = LTL_USED_VARS r) /\
+    (LTL_USED_VARS (LTL_EVENTUAL r) = LTL_USED_VARS r) /\
+    (LTL_USED_VARS (LTL_PNEXT r) = LTL_USED_VARS r) /\
+    (LTL_USED_VARS LTL_TRUE  = EMPTY) /\
+    (LTL_USED_VARS LTL_FALSE = EMPTY) /\
+    (LTL_USED_VARS LTL_INIT = EMPTY) /\
+    (LTL_USED_VARS (LTL_PALWAYS r) = LTL_USED_VARS r) /\
+    (LTL_USED_VARS (LTL_PEVENTUAL r) = LTL_USED_VARS r) /\
+    (LTL_USED_VARS (LTL_WHILE (r1,r2)) = LTL_USED_VARS r1 UNION LTL_USED_VARS r2) /\
+    (LTL_USED_VARS (LTL_BEFORE (r1,r2)) = LTL_USED_VARS r1 UNION LTL_USED_VARS r2) /\
+    (LTL_USED_VARS (LTL_SWHILE (r1,r2)) = LTL_USED_VARS r1 UNION LTL_USED_VARS r2) /\
+    (LTL_USED_VARS (LTL_SBEFORE (r1,r2)) = LTL_USED_VARS r1 UNION LTL_USED_VARS r2) /\
+    (LTL_USED_VARS (LTL_PWHILE (r1,r2)) = LTL_USED_VARS r1 UNION LTL_USED_VARS r2) /\
+    (LTL_USED_VARS (LTL_PBEFORE (r1,r2)) = LTL_USED_VARS r1 UNION LTL_USED_VARS r2) /\
+    (LTL_USED_VARS (LTL_PSWHILE (r1,r2)) = LTL_USED_VARS r1 UNION LTL_USED_VARS r2) /\
+    (LTL_USED_VARS (LTL_PSBEFORE (r1,r2)) = LTL_USED_VARS r1 UNION LTL_USED_VARS r2)
+Proof
+    SIMP_TAC std_ss [LTL_USED_VARS_def, LTL_OR_def, LTL_IMPL_def, LTL_EQUIV_def,
+                     LTL_ALWAYS_def, LTL_EVENTUAL_def, P_VAR_RENAMING_EVAL,
+                     LTL_PNEXT_def, LTL_TRUE_def, LTL_FALSE_def, LTL_INIT_def,
+                     LTL_PALWAYS_def, LTL_PEVENTUAL_def, LTL_WHILE_def,
+                     LTL_SWHILE_def, LTL_PSWHILE_def, LTL_PWHILE_def,
+                     LTL_BEFORE_def, LTL_SBEFORE_def, LTL_PSBEFORE_def,
+                     LTL_PBEFORE_def, P_USED_VARS_EVAL, UNION_EMPTY]
+ >> SIMP_TAC std_ss [EXTENSION, IN_UNION]
+ >> PROVE_TAC []
+QED
 
-  ``!l. FINITE(LTL_USED_VARS l)``,
+val LTL_VAR_RENAMING_def = Define
+  `(LTL_VAR_RENAMING f (LTL_PROP p) = LTL_PROP (P_VAR_RENAMING f p)) /\
+   (LTL_VAR_RENAMING f (LTL_NOT r) = LTL_NOT (LTL_VAR_RENAMING f r)) /\
+   (LTL_VAR_RENAMING f (LTL_AND (r1,r2)) =
+    LTL_AND(LTL_VAR_RENAMING f r1, LTL_VAR_RENAMING f r2)) /\
+   (LTL_VAR_RENAMING f (LTL_NEXT r) = LTL_NEXT (LTL_VAR_RENAMING f r)) /\
+   (LTL_VAR_RENAMING f (LTL_SUNTIL(r1,r2)) =
+    LTL_SUNTIL(LTL_VAR_RENAMING f r1, LTL_VAR_RENAMING f r2)) /\
+   (LTL_VAR_RENAMING f (LTL_PSNEXT r) = LTL_PSNEXT (LTL_VAR_RENAMING f r)) /\
+   (LTL_VAR_RENAMING f (LTL_PSUNTIL(r1,r2)) =
+    LTL_PSUNTIL(LTL_VAR_RENAMING f r1, LTL_VAR_RENAMING f r2))`;
 
-  INDUCT_THEN ltl_induct ASSUME_TAC THEN1 (
-      REWRITE_TAC[LTL_USED_VARS_def, FINITE___P_USED_VARS]
-  ) THEN
-  ASM_REWRITE_TAC[LTL_USED_VARS_def, FINITE_UNION]);
+Theorem LTL_SEM_TIME___VAR_RENAMING___NOT_INJ :
+    !f' t v f. LTL_SEM_TIME t v (LTL_VAR_RENAMING f f') =
+               LTL_SEM_TIME t (\n x. f x IN v n) f'
+Proof
+    INDUCT_THEN ltl_induct ASSUME_TAC
+ >> ASM_SIMP_TAC std_ss [LTL_VAR_RENAMING_def, LTL_SEM_TIME_def,
+                         P_SEM___VAR_RENAMING___NOT_INJ]
+QED
 
-
-val LTL_USED_VARS_EVAL=
- store_thm ("LTL_USED_VARS_EVAL",
-   ``(LTL_USED_VARS (LTL_PROP p) = P_USED_VARS p) /\
-     (LTL_USED_VARS (LTL_NOT r) = LTL_USED_VARS r) /\
-     (LTL_USED_VARS (LTL_AND (r1,r2)) = LTL_USED_VARS r1 UNION LTL_USED_VARS r2) /\
-     (LTL_USED_VARS (LTL_NEXT r) = LTL_USED_VARS r) /\
-     (LTL_USED_VARS (LTL_SUNTIL(r1,r2)) = LTL_USED_VARS r1 UNION LTL_USED_VARS r2) /\
-     (LTL_USED_VARS (LTL_PSNEXT r) = LTL_USED_VARS r) /\
-     (LTL_USED_VARS (LTL_PSUNTIL(r1,r2)) = LTL_USED_VARS r1 UNION LTL_USED_VARS r2) /\
-     (LTL_USED_VARS (LTL_OR (r1,r2)) = LTL_USED_VARS r1 UNION LTL_USED_VARS r2) /\
-     (LTL_USED_VARS (LTL_IMPL (r1,r2)) = LTL_USED_VARS r1 UNION LTL_USED_VARS r2) /\
-     (LTL_USED_VARS (LTL_EQUIV (r1,r2)) = LTL_USED_VARS r1 UNION LTL_USED_VARS r2) /\
-     (LTL_USED_VARS (LTL_ALWAYS r) = LTL_USED_VARS r) /\
-     (LTL_USED_VARS (LTL_EVENTUAL r) = LTL_USED_VARS r) /\
-     (LTL_USED_VARS (LTL_PNEXT r) = LTL_USED_VARS r) /\
-     (LTL_USED_VARS LTL_TRUE  = EMPTY) /\
-     (LTL_USED_VARS LTL_FALSE = EMPTY) /\
-     (LTL_USED_VARS LTL_INIT = EMPTY) /\
-     (LTL_USED_VARS (LTL_PALWAYS r) = LTL_USED_VARS r) /\
-     (LTL_USED_VARS (LTL_PEVENTUAL r) = LTL_USED_VARS r) /\
-     (LTL_USED_VARS (LTL_WHILE (r1,r2)) = LTL_USED_VARS r1 UNION LTL_USED_VARS r2) /\
-     (LTL_USED_VARS (LTL_BEFORE (r1,r2)) = LTL_USED_VARS r1 UNION LTL_USED_VARS r2) /\
-     (LTL_USED_VARS (LTL_SWHILE (r1,r2)) = LTL_USED_VARS r1 UNION LTL_USED_VARS r2) /\
-     (LTL_USED_VARS (LTL_SBEFORE (r1,r2)) = LTL_USED_VARS r1 UNION LTL_USED_VARS r2) /\
-     (LTL_USED_VARS (LTL_PWHILE (r1,r2)) = LTL_USED_VARS r1 UNION LTL_USED_VARS r2) /\
-     (LTL_USED_VARS (LTL_PBEFORE (r1,r2)) = LTL_USED_VARS r1 UNION LTL_USED_VARS r2) /\
-     (LTL_USED_VARS (LTL_PSWHILE (r1,r2)) = LTL_USED_VARS r1 UNION LTL_USED_VARS r2) /\
-     (LTL_USED_VARS (LTL_PSBEFORE (r1,r2)) = LTL_USED_VARS r1 UNION LTL_USED_VARS r2)``,
-
-     SIMP_TAC std_ss [LTL_USED_VARS_def, LTL_OR_def, LTL_IMPL_def, LTL_EQUIV_def,
-       LTL_ALWAYS_def, LTL_EVENTUAL_def, P_VAR_RENAMING_EVAL, LTL_PNEXT_def, LTL_TRUE_def,
-       LTL_FALSE_def, LTL_INIT_def, LTL_PALWAYS_def, LTL_PEVENTUAL_def, LTL_WHILE_def,
-       LTL_SWHILE_def, LTL_PSWHILE_def, LTL_PWHILE_def, LTL_BEFORE_def, LTL_SBEFORE_def,
-       LTL_PSBEFORE_def, LTL_PBEFORE_def, P_USED_VARS_EVAL, UNION_EMPTY] THEN
-     SIMP_TAC std_ss [EXTENSION, IN_UNION] THEN
-     PROVE_TAC[]);
-
-
-val LTL_VAR_RENAMING_def=
- Define
-   `(LTL_VAR_RENAMING f (LTL_PROP p) = LTL_PROP (P_VAR_RENAMING f p)) /\
-    (LTL_VAR_RENAMING f (LTL_NOT r) = LTL_NOT (LTL_VAR_RENAMING f r)) /\
-    (LTL_VAR_RENAMING f (LTL_AND (r1,r2)) = LTL_AND(LTL_VAR_RENAMING f r1, LTL_VAR_RENAMING f r2)) /\
-    (LTL_VAR_RENAMING f (LTL_NEXT r) = LTL_NEXT (LTL_VAR_RENAMING f r)) /\
-    (LTL_VAR_RENAMING f (LTL_SUNTIL(r1,r2)) = LTL_SUNTIL(LTL_VAR_RENAMING f r1, LTL_VAR_RENAMING f r2)) /\
-    (LTL_VAR_RENAMING f (LTL_PSNEXT r) = LTL_PSNEXT (LTL_VAR_RENAMING f r)) /\
-    (LTL_VAR_RENAMING f (LTL_PSUNTIL(r1,r2)) = LTL_PSUNTIL(LTL_VAR_RENAMING f r1, LTL_VAR_RENAMING f r2))`;
-
-
-val LTL_SEM_TIME___VAR_RENAMING___NOT_INJ =
- store_thm
-  ("LTL_SEM_TIME___VAR_RENAMING___NOT_INJ",
-   ``!f' t v f. (LTL_SEM_TIME t v (LTL_VAR_RENAMING f f')) =
-    (LTL_SEM_TIME t (\n x. f x IN v n) f')``,
-
-   INDUCT_THEN ltl_induct ASSUME_TAC THEN (
-      ASM_SIMP_TAC std_ss [LTL_VAR_RENAMING_def, LTL_SEM_TIME_def, P_SEM___VAR_RENAMING___NOT_INJ]
-   ))
-
-val LTL_SEM_TIME___VAR_RENAMING =
- store_thm
-  ("LTL_SEM_TIME___VAR_RENAMING",
-   ``!f' t v f. (INJ f (PATH_USED_VARS v UNION LTL_USED_VARS f') UNIV) ==> ((LTL_SEM_TIME t v f') = (LTL_SEM_TIME t
-    (PATH_VAR_RENAMING f v) (LTL_VAR_RENAMING f f')))``,
-
-
-   INDUCT_THEN ltl_induct ASSUME_TAC THENL [
-      SIMP_TAC std_ss [LTL_SEM_TIME_def,
-        LTL_VAR_RENAMING_def, PATH_VAR_RENAMING_def,
-        PATH_MAP_def] THEN
-      REPEAT STRIP_TAC THEN
+Theorem LTL_SEM_TIME___VAR_RENAMING :
+    !f' t v f. INJ f (PATH_USED_VARS v UNION LTL_USED_VARS f') UNIV ==>
+              (LTL_SEM_TIME t v f' =
+               LTL_SEM_TIME t (PATH_VAR_RENAMING f v) (LTL_VAR_RENAMING f f'))
+Proof
+    INDUCT_THEN ltl_induct ASSUME_TAC
+ >| [ SIMP_TAC std_ss [LTL_SEM_TIME_def,
+                       LTL_VAR_RENAMING_def, PATH_VAR_RENAMING_def,
+                       PATH_MAP_def] THEN
+      rpt STRIP_TAC THEN
       MATCH_MP_TAC P_SEM___VAR_RENAMING THEN
       UNDISCH_HD_TAC THEN
       MATCH_MP_TAC INJ_SUBSET_DOMAIN THEN
@@ -364,14 +360,12 @@ val LTL_SEM_TIME___VAR_RENAMING =
         GSYM PATH_USED_VARS_THM] THEN
       PROVE_TAC[],
 
-
       ASM_SIMP_TAC std_ss [LTL_SEM_TIME_def, LTL_USED_VARS_def,
         LTL_VAR_RENAMING_def],
 
-
       SIMP_TAC std_ss [LTL_SEM_TIME_def, LTL_USED_VARS_def,
         LTL_VAR_RENAMING_def] THEN
-      REPEAT STRIP_TAC THEN
+      rpt STRIP_TAC THEN
       REMAINS_TAC `INJ f (PATH_USED_VARS v UNION LTL_USED_VARS f'') UNIV /\
                    INJ f (PATH_USED_VARS v UNION LTL_USED_VARS f') UNIV` THEN1 (
         RES_TAC THEN
@@ -382,16 +376,14 @@ val LTL_SEM_TIME___VAR_RENAMING =
       UNDISCH_HD_TAC THEN
       MATCH_MP_TAC INJ_SUBSET_DOMAIN THEN
       SIMP_TAC std_ss [SUBSET_DEF, IN_UNION] THEN
-      PROVE_TAC[],
-
+      PROVE_TAC [],
 
       ASM_SIMP_TAC std_ss [LTL_SEM_TIME_def, LTL_USED_VARS_def,
-        LTL_VAR_RENAMING_def],
-
+                           LTL_VAR_RENAMING_def],
 
       SIMP_TAC std_ss [LTL_SEM_TIME_def, LTL_USED_VARS_def,
         LTL_VAR_RENAMING_def] THEN
-      REPEAT STRIP_TAC THEN
+      rpt STRIP_TAC THEN
       REMAINS_TAC `INJ f (PATH_USED_VARS v UNION LTL_USED_VARS f'') UNIV /\
                    INJ f (PATH_USED_VARS v UNION LTL_USED_VARS f') UNIV` THEN1 (
         RES_TAC THEN
@@ -402,8 +394,7 @@ val LTL_SEM_TIME___VAR_RENAMING =
       UNDISCH_HD_TAC THEN
       MATCH_MP_TAC INJ_SUBSET_DOMAIN THEN
       SIMP_TAC std_ss [SUBSET_DEF, IN_UNION] THEN
-      PROVE_TAC[],
-
+      PROVE_TAC [],
 
       SIMP_TAC std_ss [LTL_SEM_TIME_def, LTL_USED_VARS_def,
         LTL_VAR_RENAMING_def] THEN
@@ -412,10 +403,9 @@ val LTL_SEM_TIME___VAR_RENAMING =
         ASM_SIMP_TAC std_ss []
       ],
 
-
       SIMP_TAC std_ss [LTL_SEM_TIME_def, LTL_USED_VARS_def,
         LTL_VAR_RENAMING_def] THEN
-      REPEAT STRIP_TAC THEN
+      rpt STRIP_TAC THEN
       REMAINS_TAC `INJ f (PATH_USED_VARS v UNION LTL_USED_VARS f'') UNIV /\
                    INJ f (PATH_USED_VARS v UNION LTL_USED_VARS f') UNIV` THEN1 (
         RES_TAC THEN
@@ -426,106 +416,94 @@ val LTL_SEM_TIME___VAR_RENAMING =
       UNDISCH_HD_TAC THEN
       MATCH_MP_TAC INJ_SUBSET_DOMAIN THEN
       SIMP_TAC std_ss [SUBSET_DEF, IN_UNION] THEN
-      PROVE_TAC[]
-   ]);
+      PROVE_TAC [] ]
+QED
 
+Theorem LTL_SEM_TIME___VAR_RENAMING___PATH_RESTRICT :
+    !f' t v f. INJ f (LTL_USED_VARS f') UNIV ==>
+              (LTL_SEM_TIME t v f' =
+               LTL_SEM_TIME t (PATH_VAR_RENAMING f (PATH_RESTRICT v (LTL_USED_VARS f')))
+                              (LTL_VAR_RENAMING f f'))
+Proof
+    rpt STRIP_TAC
+ >> CONV_TAC (LHS_CONV (ONCE_REWRITE_CONV [LTL_USED_VARS_INTER_THM]))
+ >> MATCH_MP_TAC LTL_SEM_TIME___VAR_RENAMING
+ >> UNDISCH_HD_TAC
+ >> MATCH_MP_TAC INJ_SUBSET_DOMAIN
+ >> SIMP_TAC std_ss [SUBSET_DEF, IN_UNION, GSYM PATH_USED_VARS_THM,
+                     PATH_RESTRICT_def, PATH_MAP_def, IN_INTER]
+ >> PROVE_TAC []
+QED
 
+Theorem FUTURE_LTL_CONSIDERS_ONLY_FUTURE :
+    !f t v. IS_FUTURE_LTL f ==> (LTL_SEM_TIME t v f <=> LTL_SEM (\t'. v (t'+t)) f)
+Proof
+    INDUCT_THEN ltl_induct ASSUME_TAC
+ >> (SIMP_TAC std_ss [IS_FUTURE_LTL_def, LTL_SEM_TIME_def, LTL_SEM_def] \\
+     REWRITE_TAC [GSYM LTL_SEM_def] \\
+     ASM_SIMP_TAC std_ss [])
+ >| [ (* NEXT *)
+      ASM_SIMP_TAC arith_ss [arithmeticTheory.ADD1],
+      (* SUNTIL *)
+      rpt STRIP_TAC >> EQ_TAC >> rpt STRIP_TAC >| (* 2 subgoals *)
+      [ Q.EXISTS_TAC `k - t` \\
+        FULL_SIMP_TAC arith_ss [] \\
+        rpt STRIP_TAC \\
+        Q.PAT_X_ASSUM `!j. _` (MP_TAC o Q.SPEC `j+t`) \\
+        FULL_SIMP_TAC arith_ss [],
+        Q.EXISTS_TAC `k + t` \\
+        FULL_SIMP_TAC arith_ss [] \\
+        rpt STRIP_TAC \\
+        Q.PAT_X_ASSUM `!j. _` (MP_TAC o Q.SPEC `j-t`) \\
+        FULL_SIMP_TAC arith_ss [] ] ]
+QED
 
+Theorem FUTURE_LTL_EQUIVALENT_INIT_IS_EQUIVALENT :
+    !l1 l2. IS_FUTURE_LTL l1 /\ IS_FUTURE_LTL l2 ==>
+           (LTL_EQUIVALENT_INITIAL l1 l2 <=> LTL_EQUIVALENT l1 l2)
+Proof
+    SIMP_TAC std_ss [LTL_EQUIVALENT_INITIAL_def,
+                     LTL_EQUIVALENT_def, FUTURE_LTL_CONSIDERS_ONLY_FUTURE]
+ >> rpt STRIP_TAC >> EQ_TAC >> rpt STRIP_TAC
+ >- ASM_SIMP_TAC std_ss []
+ >> Q.PAT_X_ASSUM `!t w. _` (MP_TAC o Q.SPECL [`0`, `w`])
+ >> ASM_SIMP_TAC std_ss [ETA_THM]
+QED
 
-val LTL_SEM_TIME___VAR_RENAMING___PATH_RESTRICT =
- store_thm
-  ("LTL_SEM_TIME___VAR_RENAMING___PATH_RESTRICT",
-   ``!f' t v f. (INJ f (LTL_USED_VARS f') UNIV) ==> ((LTL_SEM_TIME t v f') = (LTL_SEM_TIME t
-    (PATH_VAR_RENAMING f (PATH_RESTRICT v (LTL_USED_VARS f'))) (LTL_VAR_RENAMING f f')))``,
+Theorem LTL_OR_SEM :
+    !v f1 f2 t. LTL_SEM_TIME t v (LTL_OR(f1,f2)) <=>
+                LTL_SEM_TIME t v f1 \/ LTL_SEM_TIME t v f2
+Proof
+    REWRITE_TAC [LTL_OR_def, LTL_SEM_TIME_def]
+ >> SIMP_TAC arith_ss []
+QED
 
-   REPEAT STRIP_TAC THEN
-   CONV_TAC (LHS_CONV (ONCE_REWRITE_CONV [LTL_USED_VARS_INTER_THM])) THEN
-   MATCH_MP_TAC LTL_SEM_TIME___VAR_RENAMING THEN
-   UNDISCH_HD_TAC THEN
-   MATCH_MP_TAC INJ_SUBSET_DOMAIN THEN
-   SIMP_TAC std_ss [SUBSET_DEF, IN_UNION, GSYM PATH_USED_VARS_THM,
-    PATH_RESTRICT_def, PATH_MAP_def, IN_INTER] THEN
-   PROVE_TAC[]);
+Theorem LTL_IMPL_SEM :
+    !v f1 f2 t. LTL_SEM_TIME t v (LTL_IMPL(f1,f2)) <=>
+               (LTL_SEM_TIME t v f1 ==> LTL_SEM_TIME t v f2)
+Proof
+    REWRITE_TAC [LTL_OR_def, LTL_IMPL_def, LTL_SEM_TIME_def]
+ >> METIS_TAC []
+QED
 
+Theorem LTL_EQUIV_SEM :
+    !v f1 f2 t. LTL_SEM_TIME t v (LTL_EQUIV(f1,f2)) <=>
+               (LTL_SEM_TIME t v f1 <=> LTL_SEM_TIME t v f2)
+Proof
+    REWRITE_TAC[LTL_EQUIV_def, LTL_IMPL_SEM, LTL_SEM_TIME_def]
+ >> METIS_TAC []
+QED
 
-
-val FUTURE_LTL_CONSIDERS_ONLY_FUTURE =
-  store_thm
-   ("FUTURE_LTL_CONSIDERS_ONLY_FUTURE",
-   ``!f t v. IS_FUTURE_LTL f ==> (LTL_SEM_TIME t v f <=> LTL_SEM (\t'. v (t'+t)) f)``,
-
-INDUCT_THEN ltl_induct ASSUME_TAC THEN (
-  SIMP_TAC std_ss [IS_FUTURE_LTL_def, LTL_SEM_TIME_def, LTL_SEM_def] THEN
-  REWRITE_TAC [GSYM LTL_SEM_def] THEN
-  ASM_SIMP_TAC std_ss []
-) THENL [
-  (* NEXT *)
-  ASM_SIMP_TAC arith_ss [arithmeticTheory.ADD1],
-
-  (* SUNTIL *)
-  REPEAT STRIP_TAC THEN EQ_TAC THEN REPEAT STRIP_TAC THENL [
-    Q.EXISTS_TAC `k - t` THEN
-    FULL_SIMP_TAC arith_ss [] THEN
-    REPEAT STRIP_TAC THEN
-    Q.PAT_X_ASSUM `!j. _` (MP_TAC o Q.SPEC `j+t`) THEN
-    FULL_SIMP_TAC arith_ss [],
-
-    Q.EXISTS_TAC `k + t` THEN
-    FULL_SIMP_TAC arith_ss [] THEN
-    REPEAT STRIP_TAC THEN
-    Q.PAT_X_ASSUM `!j. _` (MP_TAC o Q.SPEC `j-t`) THEN
-    FULL_SIMP_TAC arith_ss []
-  ]
-]);
-
-
-val FUTURE_LTL_EQUIVALENT_INIT_IS_EQUIVALENT =
-  store_thm
-    ("FUTURE_LTL_EQUIVALENT_INIT_IS_EQUIVALENT",
-  ``!l1 l2. IS_FUTURE_LTL l1 /\ IS_FUTURE_LTL l2 ==>
-            (LTL_EQUIVALENT_INITIAL l1 l2 <=> LTL_EQUIVALENT l1 l2)``,
-
-SIMP_TAC std_ss [LTL_EQUIVALENT_INITIAL_def,
-                 LTL_EQUIVALENT_def, FUTURE_LTL_CONSIDERS_ONLY_FUTURE] THEN
-REPEAT STRIP_TAC THEN EQ_TAC THEN REPEAT STRIP_TAC THEN1 (
-  ASM_SIMP_TAC std_ss []
-) THEN
-Q.PAT_X_ASSUM `!t w. _` (MP_TAC o Q.SPECL [`0`, `w`]) THEN
-ASM_SIMP_TAC std_ss [ETA_THM]);
-
-
-val LTL_OR_SEM =
- store_thm
-  ("LTL_OR_SEM",
-   ``!v.!f1.!f2.!t.((LTL_SEM_TIME t v (LTL_OR(f1,f2))) = ((LTL_SEM_TIME t v f1) \/ (LTL_SEM_TIME t v f2)))``,
-   REWRITE_TAC[LTL_OR_def, LTL_SEM_TIME_def] THEN SIMP_TAC arith_ss []);
-
-
-val LTL_IMPL_SEM =
- store_thm
-  ("LTL_IMPL_SEM",
-   ``!v.!f1.!f2.!t.((LTL_SEM_TIME t v (LTL_IMPL(f1,f2))) = ((LTL_SEM_TIME t v f1) ==> (LTL_SEM_TIME t v f2)))``,
-   REWRITE_TAC[LTL_OR_def, LTL_IMPL_def, LTL_SEM_TIME_def] THEN METIS_TAC[]);
-
-
-val LTL_EQUIV_SEM =
- store_thm
-  ("LTL_EQUIV_SEM",
-   ``!v.!f1.!f2.!t.((LTL_SEM_TIME t v (LTL_EQUIV(f1,f2))) = ((LTL_SEM_TIME t v f1) = (LTL_SEM_TIME t v f2)))``,
-   REWRITE_TAC[LTL_EQUIV_def, LTL_IMPL_SEM, LTL_SEM_TIME_def] THEN METIS_TAC[]);
-
-
-val LTL_SBEFORE_SEM =
- store_thm
-  ("LTL_SBEFORE_SEM",
-   ``!v.!f1.!f2.!t. ((LTL_SEM_TIME t v (LTL_SBEFORE(f1,f2))) = (
-     ?k. (k >= t /\ (LTL_SEM_TIME k v f1) /\ (!j. ((t <= j) /\ (j <= k)) ==>
-          (~(LTL_SEM_TIME j v f2))))))``,
-   REWRITE_TAC[LTL_SBEFORE_def, LTL_SEM_TIME_def] THEN
-   REPEAT STRIP_TAC THEN
+Theorem LTL_SBEFORE_SEM :
+    !v f1 f2 t. LTL_SEM_TIME t v (LTL_SBEFORE(f1,f2)) <=>
+       ?k. k >= t /\ (LTL_SEM_TIME k v f1) /\
+           !j. t <= j /\ j <= k ==> ~(LTL_SEM_TIME j v f2)
+Proof
+    REWRITE_TAC [LTL_SBEFORE_def, LTL_SEM_TIME_def]
+ >> rpt STRIP_TAC THEN
    EXISTS_EQ_STRIP_TAC THEN
-   REPEAT BOOL_EQ_STRIP_TAC THEN
-   EQ_TAC THEN REPEAT STRIP_TAC THENL [
+   rpt BOOL_EQ_STRIP_TAC THEN
+   EQ_TAC THEN rpt STRIP_TAC THENL [
      Cases_on `j < k` THENL [
        PROVE_TAC[],
 
@@ -538,264 +516,230 @@ val LTL_SBEFORE_SEM =
 
      `j <= k` by DECIDE_TAC THEN
      PROVE_TAC[]
-   ]);
+   ]
+QED
 
-
-val LTL_PSBEFORE_SEM =
- store_thm
-  ("LTL_PSBEFORE_SEM",
-   ``!v.!f1.!f2.!t. ((LTL_SEM_TIME t v (LTL_PSBEFORE(f1,f2))) = (
-     ?k. (k <= t /\ (LTL_SEM_TIME k v f1) /\ (!j. ((k <= j) /\ (j <= t)) ==>
-          (~(LTL_SEM_TIME j v f2))))))``,
-   REWRITE_TAC[LTL_PSBEFORE_def, LTL_SEM_TIME_def] THEN
-   REPEAT STRIP_TAC THEN
-   EXISTS_EQ_STRIP_TAC THEN
-   REPEAT BOOL_EQ_STRIP_TAC THEN
-   EQ_TAC THEN REPEAT STRIP_TAC THENL [
-     Cases_on `k < j` THENL [
-       PROVE_TAC[],
-
+Theorem LTL_PSBEFORE_SEM :
+    !v f1 f2 t. LTL_SEM_TIME t v (LTL_PSBEFORE(f1,f2)) <=>
+                ?k. k <= t /\ LTL_SEM_TIME k v f1 /\
+                    !j. k <= j /\ j <= t ==> ~(LTL_SEM_TIME j v f2)
+Proof
+    REWRITE_TAC [LTL_PSBEFORE_def, LTL_SEM_TIME_def]
+ >> rpt STRIP_TAC
+ >> EXISTS_EQ_STRIP_TAC
+ >> rpt BOOL_EQ_STRIP_TAC
+ >> EQ_TAC >> rpt STRIP_TAC
+ >| [ Cases_on `k < j` THENL [
+       PROVE_TAC [],
        `j = k` by DECIDE_TAC THEN
-       PROVE_TAC[]
-     ],
+       PROVE_TAC []
+      ],
 
      `k <= k` by DECIDE_TAC THEN
-     PROVE_TAC[],
+      PROVE_TAC [],
 
      `k <= j` by DECIDE_TAC THEN
-     PROVE_TAC[]
-   ]);
+      PROVE_TAC [] ]
+QED
 
+Theorem LTL_EVENTUAL_SEM :
+    !v f t. LTL_SEM_TIME t v (LTL_EVENTUAL f) = ?k. k >= t /\ LTL_SEM_TIME k v f
+Proof
+    EVAL_TAC >> SIMP_TAC arith_ss [P_SEM_THM]
+QED
 
-val LTL_EVENTUAL_SEM =
- store_thm
-  ("LTL_EVENTUAL_SEM",
-   ``!v.!f.!t.(LTL_SEM_TIME t v (LTL_EVENTUAL f) =  (?k. (k >= t) /\ (LTL_SEM_TIME k v f)))``,
-   EVAL_TAC THEN SIMP_TAC arith_ss [P_SEM_THM]);
+Theorem LTL_ALWAYS_SEM :
+    !v f t. LTL_SEM_TIME t v (LTL_ALWAYS f) = !k. k >= t ==> LTL_SEM_TIME k v f
+Proof
+    EVAL_TAC >> SIMP_TAC arith_ss [P_SEM_THM]
+ >> PROVE_TAC []
+QED
 
+Theorem LTL_PEVENTUAL_SEM :
+    !v f t. LTL_SEM_TIME t v (LTL_PEVENTUAL f) =
+            ?k:num. (0 <= k /\ k <= t) /\ LTL_SEM_TIME k v f
+Proof
+    EVAL_TAC >> SIMP_TAC arith_ss [P_SEM_THM]
+QED
 
-val LTL_ALWAYS_SEM =
- store_thm
-  ("LTL_ALWAYS_SEM",
-   ``!v.!f.!t. (LTL_SEM_TIME t v (LTL_ALWAYS f) = (!k. (k >= t) ==> (LTL_SEM_TIME k v f)))``,
-   EVAL_TAC THEN SIMP_TAC arith_ss [P_SEM_THM] THEN
-   PROVE_TAC[]);
+Theorem LTL_PALWAYS_SEM :
+    !v f t. LTL_SEM_TIME t v (LTL_PALWAYS f) = !k. k <= t ==> LTL_SEM_TIME k v f
+Proof
+    EVAL_TAC >> SIMP_TAC arith_ss [P_SEM_THM] >> PROVE_TAC []
+QED
 
+Theorem LTL_PNEXT_SEM :
+    !v f t. LTL_SEM_TIME t v (LTL_PNEXT f) = ((t = 0) \/ LTL_SEM_TIME (PRE t) v f)
+Proof
+    EVAL_TAC >> SIMP_TAC arith_ss [P_SEM_THM]
+ >> `!t:num. (~(t > 0)) = (t = 0)` by DECIDE_TAC
+ >> PROVE_TAC []
+QED
 
-val LTL_PEVENTUAL_SEM =
- store_thm
-  ("LTL_PEVENTUAL_SEM",
-   ``!v.!f.!t.(LTL_SEM_TIME t v (LTL_PEVENTUAL f) = (?k:num. (0 <= k /\ k <= t) /\ (LTL_SEM_TIME k v f)))``,
-   EVAL_TAC THEN SIMP_TAC arith_ss [P_SEM_THM]);
+Theorem LTL_TRUE_SEM :
+    !v t. LTL_SEM_TIME t v LTL_TRUE
+Proof
+    REWRITE_TAC [LTL_TRUE_def, LTL_SEM_TIME_def, P_SEM_THM]
+QED
 
+Theorem LTL_FALSE_SEM :
+    !v t. ~(LTL_SEM_TIME t v LTL_FALSE)
+Proof
+    REWRITE_TAC [LTL_FALSE_def, LTL_SEM_TIME_def, P_SEM_THM]
+QED
 
-val LTL_PALWAYS_SEM =
- store_thm
-  ("LTL_PALWAYS_SEM",
-   ``!v.!f.!t. (LTL_SEM_TIME t v (LTL_PALWAYS f) = (!k. (k <= t) ==> (LTL_SEM_TIME k v f)))``,
-   EVAL_TAC THEN SIMP_TAC arith_ss [P_SEM_THM] THEN
-   PROVE_TAC[]);
+Theorem LTL_INIT_SEM :
+    !t v. (LTL_SEM_TIME t v LTL_INIT) = (t = 0)
+Proof
+    REWRITE_TAC [LTL_INIT_def, LTL_SEM_TIME_def, P_SEM_def]
+ >> DECIDE_TAC
+QED
 
+Theorem LTL_SEM_THM = LIST_CONJ
+   [LTL_SEM_def, LTL_SEM_TIME_def,
+    LTL_OR_SEM,
+    LTL_IMPL_SEM,
+    LTL_EQUIV_SEM,
+    LTL_ALWAYS_SEM,
+    LTL_EVENTUAL_SEM,
+    LTL_PNEXT_SEM,
+    LTL_PEVENTUAL_SEM,
+    LTL_PALWAYS_SEM,
+    LTL_TRUE_SEM,
+    LTL_FALSE_SEM,
+    LTL_INIT_SEM,
+    LTL_SBEFORE_SEM,
+    LTL_PSBEFORE_SEM];
 
-val LTL_PNEXT_SEM =
- store_thm
-  ("LTL_PNEXT_SEM",
-   ``!v.!f.!t. (LTL_SEM_TIME t v (LTL_PNEXT f) = ((t = 0) \/  LTL_SEM_TIME (PRE t) v f))``,
-   EVAL_TAC THEN SIMP_TAC arith_ss [P_SEM_THM] THEN
-   `!t:num. (~(t > 0)) = (t = 0)` by DECIDE_TAC THEN
-   PROVE_TAC[]);
+Theorem LTL_VAR_RENAMING_EVAL :
+    (LTL_VAR_RENAMING f (LTL_PROP p) = LTL_PROP (P_VAR_RENAMING f p)) /\
+    (LTL_VAR_RENAMING f (LTL_NOT r) = LTL_NOT (LTL_VAR_RENAMING f r)) /\
+    (LTL_VAR_RENAMING f (LTL_AND (r1,r2)) = LTL_AND(LTL_VAR_RENAMING f r1, LTL_VAR_RENAMING f r2)) /\
+    (LTL_VAR_RENAMING f (LTL_NEXT r) = LTL_NEXT (LTL_VAR_RENAMING f r)) /\
+    (LTL_VAR_RENAMING f (LTL_SUNTIL(r1,r2)) = LTL_SUNTIL(LTL_VAR_RENAMING f r1, LTL_VAR_RENAMING f r2)) /\
+    (LTL_VAR_RENAMING f (LTL_PSNEXT r) = LTL_PSNEXT (LTL_VAR_RENAMING f r)) /\
+    (LTL_VAR_RENAMING f (LTL_PSUNTIL(r1,r2)) = LTL_PSUNTIL(LTL_VAR_RENAMING f r1, LTL_VAR_RENAMING f r2)) /\
+    (LTL_VAR_RENAMING f (LTL_OR (r1,r2)) = LTL_OR(LTL_VAR_RENAMING f r1, LTL_VAR_RENAMING f r2)) /\
+    (LTL_VAR_RENAMING f (LTL_IMPL (r1,r2)) = LTL_IMPL(LTL_VAR_RENAMING f r1, LTL_VAR_RENAMING f r2)) /\
+    (LTL_VAR_RENAMING f (LTL_EQUIV (r1,r2)) = LTL_EQUIV(LTL_VAR_RENAMING f r1, LTL_VAR_RENAMING f r2)) /\
+    (LTL_VAR_RENAMING f (LTL_ALWAYS r) = LTL_ALWAYS (LTL_VAR_RENAMING f r)) /\
+    (LTL_VAR_RENAMING f (LTL_EVENTUAL r) = LTL_EVENTUAL (LTL_VAR_RENAMING f r)) /\
+    (LTL_VAR_RENAMING f (LTL_PNEXT r) = LTL_PNEXT (LTL_VAR_RENAMING f r)) /\
+    (LTL_VAR_RENAMING f LTL_TRUE  = LTL_TRUE) /\
+    (LTL_VAR_RENAMING f LTL_FALSE = LTL_FALSE) /\
+    (LTL_VAR_RENAMING f LTL_INIT = LTL_INIT) /\
+    (LTL_VAR_RENAMING f (LTL_PALWAYS r) = LTL_PALWAYS (LTL_VAR_RENAMING f r)) /\
+    (LTL_VAR_RENAMING f (LTL_PEVENTUAL r) = LTL_PEVENTUAL (LTL_VAR_RENAMING f r)) /\
+    (LTL_VAR_RENAMING f (LTL_WHILE (r1,r2)) = LTL_WHILE(LTL_VAR_RENAMING f r1, LTL_VAR_RENAMING f r2)) /\
+    (LTL_VAR_RENAMING f (LTL_BEFORE (r1,r2)) = LTL_BEFORE(LTL_VAR_RENAMING f r1, LTL_VAR_RENAMING f r2)) /\
+    (LTL_VAR_RENAMING f (LTL_SWHILE (r1,r2)) = LTL_SWHILE(LTL_VAR_RENAMING f r1, LTL_VAR_RENAMING f r2)) /\
+    (LTL_VAR_RENAMING f (LTL_SBEFORE (r1,r2)) = LTL_SBEFORE(LTL_VAR_RENAMING f r1, LTL_VAR_RENAMING f r2)) /\
+    (LTL_VAR_RENAMING f (LTL_PWHILE (r1,r2)) = LTL_PWHILE(LTL_VAR_RENAMING f r1, LTL_VAR_RENAMING f r2)) /\
+    (LTL_VAR_RENAMING f (LTL_PBEFORE (r1,r2)) = LTL_PBEFORE(LTL_VAR_RENAMING f r1, LTL_VAR_RENAMING f r2)) /\
+    (LTL_VAR_RENAMING f (LTL_PSWHILE (r1,r2)) = LTL_PSWHILE(LTL_VAR_RENAMING f r1, LTL_VAR_RENAMING f r2)) /\
+    (LTL_VAR_RENAMING f (LTL_PSBEFORE (r1,r2)) = LTL_PSBEFORE(LTL_VAR_RENAMING f r1, LTL_VAR_RENAMING f r2))
+Proof
+    SIMP_TAC std_ss [LTL_VAR_RENAMING_def, LTL_OR_def, LTL_IMPL_def, LTL_EQUIV_def,
+                     LTL_ALWAYS_def, LTL_EVENTUAL_def, P_VAR_RENAMING_EVAL,
+                     LTL_PNEXT_def, LTL_TRUE_def, LTL_FALSE_def, LTL_INIT_def,
+                     LTL_PALWAYS_def, LTL_PEVENTUAL_def, LTL_WHILE_def,
+                     LTL_SWHILE_def, LTL_PSWHILE_def, LTL_PWHILE_def, LTL_BEFORE_def,
+                     LTL_SBEFORE_def, LTL_PSBEFORE_def, LTL_PBEFORE_def]
+QED
 
-val LTL_TRUE_SEM =
- store_thm
-  ("LTL_TRUE_SEM",
-   ``!v t. LTL_SEM_TIME t v LTL_TRUE``,
-   REWRITE_TAC[LTL_TRUE_def, LTL_SEM_TIME_def, P_SEM_THM]);
+(* LTL_ALWAYS is usually defined as NOT EVENTUAL. However, this is simplified by
+   the nnf rewrites defined in temporal_deep_simplifiactionsLib to ALWAYS again.
+   Thus, the simplifier may loop. Therefore, here are direct definitions of ALWAYS
+   and PALWAYS to use with the nnf rewrites.
+ *)
+Theorem LTL_ALWAYS_PALWAYS_ALTERNATIVE_DEFS :
+    (!l. LTL_ALWAYS l = LTL_NOT (LTL_SUNTIL (LTL_TRUE, LTL_NOT l))) /\
+    (!l. LTL_PALWAYS l = LTL_NOT (LTL_PSUNTIL (LTL_TRUE, LTL_NOT l)))
+Proof
+    SIMP_TAC std_ss [LTL_ALWAYS_def, LTL_EVENTUAL_def, LTL_TRUE_def,
+                     LTL_PALWAYS_def, LTL_PEVENTUAL_def]
+QED
 
+val LTL_IS_CONTRADICTION_def = Define
+   `LTL_IS_CONTRADICTION l = !v. ~(LTL_SEM v l)`;
 
-val LTL_FALSE_SEM =
- store_thm
-  ("LTL_FALSE_SEM",
-   ``!v t. ~(LTL_SEM_TIME t v LTL_FALSE)``,
-   REWRITE_TAC[LTL_FALSE_def, LTL_SEM_TIME_def, P_SEM_THM]);
+val LTL_IS_TAUTOLOGY_def = Define
+   `LTL_IS_TAUTOLOGY l = !v. LTL_SEM v l`;
 
+Theorem LTL_TAUTOLOGY_CONTRADICTION_DUAL :
+    (!l. LTL_IS_CONTRADICTION (LTL_NOT l) <=> LTL_IS_TAUTOLOGY l) /\
+    (!l. LTL_IS_TAUTOLOGY (LTL_NOT l) <=> LTL_IS_CONTRADICTION l)
+Proof
+    REWRITE_TAC [LTL_IS_TAUTOLOGY_def, LTL_IS_CONTRADICTION_def,
+                 LTL_SEM_TIME_def, LTL_SEM_def]
+QED
 
-val LTL_INIT_SEM =
- store_thm
-  ("LTL_INIT_SEM",
-   ``!t v. (LTL_SEM_TIME t v LTL_INIT) = (t = 0)``,
+Theorem LTL_TAUTOLOGY_CONTRADICTION___TO___EQUIVALENT_INITIAL :
+    (!l. LTL_IS_CONTRADICTION l <=> LTL_EQUIVALENT_INITIAL l LTL_FALSE) /\
+    (!l. LTL_IS_TAUTOLOGY l <=> LTL_EQUIVALENT_INITIAL l LTL_TRUE)
+Proof
+    REWRITE_TAC [LTL_IS_TAUTOLOGY_def, LTL_IS_CONTRADICTION_def, LTL_SEM_THM,
+                 LTL_EQUIVALENT_INITIAL_def]
+ >> PROVE_TAC []
+QED
 
-   REWRITE_TAC[LTL_INIT_def, LTL_SEM_TIME_def, P_SEM_def] THEN
-   DECIDE_TAC);
+Theorem LTL_EQUIVALENT_INITIAL___TO___TAUTOLOGY :
+    !l1 l2. LTL_EQUIVALENT_INITIAL l1 l2 <=> LTL_IS_TAUTOLOGY (LTL_EQUIV(l1, l2))
+Proof
+    REWRITE_TAC [LTL_IS_TAUTOLOGY_def, LTL_SEM_THM,
+                 LTL_EQUIVALENT_INITIAL_def]
+ >> PROVE_TAC []
+QED
 
+Theorem LTL_EQUIVALENT_INITIAL___TO___CONTRADICTION :
+    !l1 l2. LTL_EQUIVALENT_INITIAL l1 l2 <=>
+            LTL_IS_CONTRADICTION (LTL_NOT (LTL_EQUIV(l1, l2)))
+Proof
+    REWRITE_TAC [LTL_TAUTOLOGY_CONTRADICTION_DUAL,
+                 LTL_EQUIVALENT_INITIAL___TO___TAUTOLOGY]
+QED
 
-val LTL_SEM_THM = LIST_CONJ [LTL_SEM_def,
-                             LTL_SEM_TIME_def,
-                             LTL_OR_SEM,
-                             LTL_IMPL_SEM,
-                             LTL_EQUIV_SEM,
-                             LTL_ALWAYS_SEM,
-                             LTL_EVENTUAL_SEM,
-                             LTL_PNEXT_SEM,
-                             LTL_PEVENTUAL_SEM,
-                             LTL_PALWAYS_SEM,
-                             LTL_TRUE_SEM,
-                             LTL_FALSE_SEM,
-                             LTL_INIT_SEM,
-                             LTL_SBEFORE_SEM,
-                             LTL_PSBEFORE_SEM];
-val _ = save_thm("LTL_SEM_THM",LTL_SEM_THM);
+Theorem LTL_EQUIVALENT___TO___CONTRADICTION :
+    !l1 l2. LTL_EQUIVALENT l1 l2 <=>
+            LTL_IS_CONTRADICTION (LTL_EVENTUAL (LTL_NOT (LTL_EQUIV (l1,l2))))
+Proof
+    SIMP_TAC std_ss [LTL_EQUIVALENT_def, LTL_IS_CONTRADICTION_def, LTL_SEM_THM]
+ >> PROVE_TAC []
+QED
 
+Theorem LTL_CONTRADICTION___VAR_RENAMING :
+    !f' f. INJ f (LTL_USED_VARS f') UNIV ==>
+          (LTL_IS_CONTRADICTION f' <=> LTL_IS_CONTRADICTION (LTL_VAR_RENAMING f f'))
+Proof
+    SIMP_TAC std_ss [LTL_IS_CONTRADICTION_def, LTL_SEM_def]
+ >> rpt STRIP_TAC >> EQ_TAC
+ >| [ SIMP_TAC std_ss [LTL_SEM_TIME___VAR_RENAMING___NOT_INJ],
+      PROVE_TAC[LTL_SEM_TIME___VAR_RENAMING___PATH_RESTRICT] ]
+QED
 
-val LTL_VAR_RENAMING_EVAL=
- store_thm ("LTL_VAR_RENAMING_EVAL",
-   ``(LTL_VAR_RENAMING f (LTL_PROP p) = LTL_PROP (P_VAR_RENAMING f p)) /\
-     (LTL_VAR_RENAMING f (LTL_NOT r) = LTL_NOT (LTL_VAR_RENAMING f r)) /\
-     (LTL_VAR_RENAMING f (LTL_AND (r1,r2)) = LTL_AND(LTL_VAR_RENAMING f r1, LTL_VAR_RENAMING f r2)) /\
-     (LTL_VAR_RENAMING f (LTL_NEXT r) = LTL_NEXT (LTL_VAR_RENAMING f r)) /\
-     (LTL_VAR_RENAMING f (LTL_SUNTIL(r1,r2)) = LTL_SUNTIL(LTL_VAR_RENAMING f r1, LTL_VAR_RENAMING f r2)) /\
-     (LTL_VAR_RENAMING f (LTL_PSNEXT r) = LTL_PSNEXT (LTL_VAR_RENAMING f r)) /\
-     (LTL_VAR_RENAMING f (LTL_PSUNTIL(r1,r2)) = LTL_PSUNTIL(LTL_VAR_RENAMING f r1, LTL_VAR_RENAMING f r2)) /\
-     (LTL_VAR_RENAMING f (LTL_OR (r1,r2)) = LTL_OR(LTL_VAR_RENAMING f r1, LTL_VAR_RENAMING f r2)) /\
-     (LTL_VAR_RENAMING f (LTL_IMPL (r1,r2)) = LTL_IMPL(LTL_VAR_RENAMING f r1, LTL_VAR_RENAMING f r2)) /\
-     (LTL_VAR_RENAMING f (LTL_EQUIV (r1,r2)) = LTL_EQUIV(LTL_VAR_RENAMING f r1, LTL_VAR_RENAMING f r2)) /\
-     (LTL_VAR_RENAMING f (LTL_ALWAYS r) = LTL_ALWAYS (LTL_VAR_RENAMING f r)) /\
-     (LTL_VAR_RENAMING f (LTL_EVENTUAL r) = LTL_EVENTUAL (LTL_VAR_RENAMING f r)) /\
-     (LTL_VAR_RENAMING f (LTL_PNEXT r) = LTL_PNEXT (LTL_VAR_RENAMING f r)) /\
-     (LTL_VAR_RENAMING f LTL_TRUE  = LTL_TRUE) /\
-     (LTL_VAR_RENAMING f LTL_FALSE = LTL_FALSE) /\
-     (LTL_VAR_RENAMING f LTL_INIT = LTL_INIT) /\
-     (LTL_VAR_RENAMING f (LTL_PALWAYS r) = LTL_PALWAYS (LTL_VAR_RENAMING f r)) /\
-     (LTL_VAR_RENAMING f (LTL_PEVENTUAL r) = LTL_PEVENTUAL (LTL_VAR_RENAMING f r)) /\
-     (LTL_VAR_RENAMING f (LTL_WHILE (r1,r2)) = LTL_WHILE(LTL_VAR_RENAMING f r1, LTL_VAR_RENAMING f r2)) /\
-     (LTL_VAR_RENAMING f (LTL_BEFORE (r1,r2)) = LTL_BEFORE(LTL_VAR_RENAMING f r1, LTL_VAR_RENAMING f r2)) /\
-     (LTL_VAR_RENAMING f (LTL_SWHILE (r1,r2)) = LTL_SWHILE(LTL_VAR_RENAMING f r1, LTL_VAR_RENAMING f r2)) /\
-     (LTL_VAR_RENAMING f (LTL_SBEFORE (r1,r2)) = LTL_SBEFORE(LTL_VAR_RENAMING f r1, LTL_VAR_RENAMING f r2)) /\
-     (LTL_VAR_RENAMING f (LTL_PWHILE (r1,r2)) = LTL_PWHILE(LTL_VAR_RENAMING f r1, LTL_VAR_RENAMING f r2)) /\
-     (LTL_VAR_RENAMING f (LTL_PBEFORE (r1,r2)) = LTL_PBEFORE(LTL_VAR_RENAMING f r1, LTL_VAR_RENAMING f r2)) /\
-     (LTL_VAR_RENAMING f (LTL_PSWHILE (r1,r2)) = LTL_PSWHILE(LTL_VAR_RENAMING f r1, LTL_VAR_RENAMING f r2)) /\
-     (LTL_VAR_RENAMING f (LTL_PSBEFORE (r1,r2)) = LTL_PSBEFORE(LTL_VAR_RENAMING f r1, LTL_VAR_RENAMING f r2))``,
-
-     SIMP_TAC std_ss [LTL_VAR_RENAMING_def, LTL_OR_def, LTL_IMPL_def, LTL_EQUIV_def,
-       LTL_ALWAYS_def, LTL_EVENTUAL_def, P_VAR_RENAMING_EVAL, LTL_PNEXT_def, LTL_TRUE_def,
-       LTL_FALSE_def, LTL_INIT_def, LTL_PALWAYS_def, LTL_PEVENTUAL_def, LTL_WHILE_def,
-       LTL_SWHILE_def, LTL_PSWHILE_def, LTL_PWHILE_def, LTL_BEFORE_def, LTL_SBEFORE_def,
-       LTL_PSBEFORE_def, LTL_PBEFORE_def]);
-
-
-(*LTL_ALWAYS is usually defined as NOT EVENTUAL. However, this is simplified by
-  the nnf rewrites defined in temporal_deep_simplifiactionsLib to ALWAYS again. Thus, the simplifier may loop. Therefore, here are
-  direct definitions of ALWAYS and PALWAYS to use with the nnf rewrites*)
-val LTL_ALWAYS_PALWAYS_ALTERNATIVE_DEFS =
-  store_thm (
-    "LTL_ALWAYS_PALWAYS_ALTERNATIVE_DEFS",
-    ``(!l. (LTL_ALWAYS l) = (LTL_NOT (LTL_SUNTIL (LTL_TRUE, LTL_NOT l)))) /\
-      (!l. (LTL_PALWAYS l) = (LTL_NOT (LTL_PSUNTIL (LTL_TRUE, LTL_NOT l))))``,
-
-      SIMP_TAC std_ss [LTL_ALWAYS_def, LTL_EVENTUAL_def, LTL_TRUE_def,
-                       LTL_PALWAYS_def, LTL_PEVENTUAL_def]);
-
-
-val LTL_IS_CONTRADICTION_def =
- Define
-   `LTL_IS_CONTRADICTION l = (!v. ~(LTL_SEM v l))`;
-
-val LTL_IS_TAUTOLOGY_def =
- Define
-   `LTL_IS_TAUTOLOGY l = (!v. LTL_SEM v l)`;
-
-
-val LTL_TAUTOLOGY_CONTRADICTION_DUAL =
- store_thm
-  ("LTL_TAUTOLOGY_CONTRADICTION_DUAL",
-
-  ``(!l. LTL_IS_CONTRADICTION (LTL_NOT l) = LTL_IS_TAUTOLOGY l) /\
-    (!l. LTL_IS_TAUTOLOGY (LTL_NOT l) = LTL_IS_CONTRADICTION l)``,
-
-    REWRITE_TAC[LTL_IS_TAUTOLOGY_def, LTL_IS_CONTRADICTION_def, LTL_SEM_TIME_def,
-      LTL_SEM_def]);
-
-
-val LTL_TAUTOLOGY_CONTRADICTION___TO___EQUIVALENT_INITIAL =
- store_thm
-  ("LTL_TAUTOLOGY_CONTRADICTION___TO___EQUIVALENT_INITIAL",
-
-  ``(!l. LTL_IS_CONTRADICTION l = LTL_EQUIVALENT_INITIAL l LTL_FALSE) /\
-    (!l. LTL_IS_TAUTOLOGY l = LTL_EQUIVALENT_INITIAL l LTL_TRUE)``,
-
-    REWRITE_TAC[LTL_IS_TAUTOLOGY_def, LTL_IS_CONTRADICTION_def, LTL_SEM_THM,
-      LTL_EQUIVALENT_INITIAL_def] THEN
-    PROVE_TAC[]);
-
-
-val LTL_EQUIVALENT_INITIAL___TO___TAUTOLOGY =
- store_thm
-  ("LTL_EQUIVALENT_INITIAL___TO___TAUTOLOGY",
-
-  ``!l1 l2. LTL_EQUIVALENT_INITIAL l1 l2 = LTL_IS_TAUTOLOGY (LTL_EQUIV(l1, l2))``,
-
-    REWRITE_TAC[LTL_IS_TAUTOLOGY_def, LTL_SEM_THM,
-      LTL_EQUIVALENT_INITIAL_def] THEN
-    PROVE_TAC[]);
-
-val LTL_EQUIVALENT_INITIAL___TO___CONTRADICTION =
- store_thm
-  ("LTL_EQUIVALENT_INITIAL___TO___CONTRADICTION",
-
-  ``!l1 l2. LTL_EQUIVALENT_INITIAL l1 l2 = LTL_IS_CONTRADICTION (LTL_NOT (LTL_EQUIV(l1, l2)))``,
-
-    REWRITE_TAC[LTL_TAUTOLOGY_CONTRADICTION_DUAL,
-        LTL_EQUIVALENT_INITIAL___TO___TAUTOLOGY]);
-
-val LTL_EQUIVALENT___TO___CONTRADICTION =
- store_thm
-  ("LTL_EQUIVALENT___TO___CONTRADICTION",
-
-  ``!l1 l2. LTL_EQUIVALENT l1 l2 =
-        LTL_IS_CONTRADICTION (LTL_EVENTUAL (LTL_NOT (LTL_EQUIV (l1,l2))))``,
-
-    SIMP_TAC std_ss [LTL_EQUIVALENT_def, LTL_IS_CONTRADICTION_def,
-                    LTL_SEM_THM] THEN
-    PROVE_TAC[]);
-
-
-val LTL_CONTRADICTION___VAR_RENAMING =
- store_thm
-  ("LTL_CONTRADICTION___VAR_RENAMING",
-   ``!f' f. (INJ f (LTL_USED_VARS f') UNIV) ==> (LTL_IS_CONTRADICTION f' = LTL_IS_CONTRADICTION (LTL_VAR_RENAMING f f'))``,
-
-   SIMP_TAC std_ss [LTL_IS_CONTRADICTION_def,
-     LTL_SEM_def] THEN
-   REPEAT STRIP_TAC THEN EQ_TAC THENL [
-     SIMP_TAC std_ss [LTL_SEM_TIME___VAR_RENAMING___NOT_INJ],
-     PROVE_TAC[LTL_SEM_TIME___VAR_RENAMING___PATH_RESTRICT]
-   ]);
-
-
-val LTL_KS_SEM___VAR_RENAMING =
- store_thm
-  ("LTL_KS_SEM___VAR_RENAMING",
-   ``!f' M f. (INJ f (LTL_USED_VARS f' UNION (SYMBOLIC_KRIPKE_STRUCTURE_USED_VARS M)) UNIV) ==> (LTL_KS_SEM M f' = LTL_KS_SEM
-      (SYMBOLIC_KRIPKE_STRUCTURE_VAR_RENAMING f M)
-      (LTL_VAR_RENAMING f f'))``,
-
-   SIMP_TAC std_ss [LTL_KS_SEM_def, LTL_SEM_def,
-                    PATHS_THROUGH_SYMBOLIC_KRIPKE_STRUCTURE___REWRITES,
-                    SYMBOLIC_KRIPKE_STRUCTURE_VAR_RENAMING_def,
-                    symbolic_kripke_structure_REWRITES] THEN
-   REPEAT STRIP_TAC THEN EQ_TAC THEN REPEAT STRIP_TAC THENL [
-      SIMP_ALL_TAC std_ss [P_SEM___VAR_RENAMING___NOT_INJ,
+Theorem LTL_KS_SEM___VAR_RENAMING :
+    !f' M f. INJ f (LTL_USED_VARS f' UNION (SYMBOLIC_KRIPKE_STRUCTURE_USED_VARS M)) UNIV ==>
+            (LTL_KS_SEM M f' <=> LTL_KS_SEM (SYMBOLIC_KRIPKE_STRUCTURE_VAR_RENAMING f M)
+                                            (LTL_VAR_RENAMING f f'))
+Proof
+    SIMP_TAC std_ss [LTL_KS_SEM_def, LTL_SEM_def,
+                     PATHS_THROUGH_SYMBOLIC_KRIPKE_STRUCTURE___REWRITES,
+                     SYMBOLIC_KRIPKE_STRUCTURE_VAR_RENAMING_def,
+                     symbolic_kripke_structure_REWRITES]
+ >> rpt STRIP_TAC >> EQ_TAC >> rpt STRIP_TAC
+ >| [ SIMP_ALL_TAC std_ss [P_SEM___VAR_RENAMING___NOT_INJ,
                            XP_SEM___VAR_RENAMING___NOT_INJ,
                            LTL_SEM_TIME___VAR_RENAMING___NOT_INJ] THEN
       Q_SPEC_NO_ASSUM 2 `(\n x. f x IN p n)` THEN
       UNDISCH_HD_TAC THEN
       ASM_SIMP_TAC std_ss [],
 
-
-      `?w. w = PATH_RESTRICT p (LTL_USED_VARS f' UNION SYMBOLIC_KRIPKE_STRUCTURE_USED_VARS M)` by PROVE_TAC[] THEN
+     `?w. w = PATH_RESTRICT p (LTL_USED_VARS f' UNION
+      SYMBOLIC_KRIPKE_STRUCTURE_USED_VARS M)` by PROVE_TAC [] THEN
       SUBGOAL_TAC `(LTL_SEM_TIME 0 p f' = LTL_SEM_TIME 0 w f') /\
                    (P_SEM (p 0) M.S0 = P_SEM (w 0) M.S0) /\
                    !n. (XP_SEM M.R (p n,p (SUC n)) = XP_SEM M.R (w n,w (SUC n)))` THEN1 (
-        REPEAT STRIP_TAC THENL [
+        rpt STRIP_TAC THENL [
           ASM_REWRITE_TAC[] THEN
           MATCH_MP_TAC LTL_USED_VARS_INTER_SUBSET_THM THEN
           SIMP_TAC std_ss [SUBSET_UNION],
@@ -815,12 +759,11 @@ val LTL_KS_SEM___VAR_RENAMING =
             IN_UNION]
         ]
       ) THEN
-      `!n. w n SUBSET (LTL_USED_VARS f' UNION SYMBOLIC_KRIPKE_STRUCTURE_USED_VARS M)` by METIS_TAC[PATH_RESTRICT_SUBSET] THEN
+      `!n. w n SUBSET (LTL_USED_VARS f' UNION
+                       SYMBOLIC_KRIPKE_STRUCTURE_USED_VARS M)`
+          by METIS_TAC[PATH_RESTRICT_SUBSET] THEN
       GSYM_NO_TAC 4 THEN
-
       FULL_SIMP_TAC std_ss [] THEN NTAC 3 (WEAKEN_NO_TAC 2) THEN
-
-
       Q_SPEC_NO_ASSUM 4 `PATH_VAR_RENAMING f w` THEN
       UNDISCH_HD_TAC THEN
       REMAINS_TAC `(!n.
@@ -834,15 +777,14 @@ val LTL_KS_SEM___VAR_RENAMING =
         FULL_SIMP_TAC std_ss []
       ) THEN
 
-      REPEAT STRIP_TAC THENL [
+      rpt STRIP_TAC THENL [
         SIMP_TAC std_ss [PATH_VAR_RENAMING_def, PATH_MAP_def] THEN
         MATCH_MP_TAC (GSYM XP_SEM___VAR_RENAMING) THEN
         UNDISCH_NO_TAC 4 THEN
         MATCH_MP_TAC INJ_SUBSET_DOMAIN THEN
         SIMP_ALL_TAC std_ss [SYMBOLIC_KRIPKE_STRUCTURE_USED_VARS_def,
                          IN_UNION, SUBSET_DEF] THEN
-        PROVE_TAC[],
-
+        PROVE_TAC [],
 
         SIMP_TAC std_ss [PATH_VAR_RENAMING_def, PATH_MAP_def] THEN
         MATCH_MP_TAC (GSYM P_SEM___VAR_RENAMING) THEN
@@ -850,87 +792,63 @@ val LTL_KS_SEM___VAR_RENAMING =
         MATCH_MP_TAC INJ_SUBSET_DOMAIN THEN
         SIMP_ALL_TAC std_ss [SYMBOLIC_KRIPKE_STRUCTURE_USED_VARS_def,
                          IN_UNION, SUBSET_DEF] THEN
-        PROVE_TAC[],
-
+        PROVE_TAC [],
 
         MATCH_MP_TAC (GSYM LTL_SEM_TIME___VAR_RENAMING) THEN
         UNDISCH_NO_TAC 4 THEN
         MATCH_MP_TAC INJ_SUBSET_DOMAIN THEN
         SIMP_ALL_TAC std_ss [SYMBOLIC_KRIPKE_STRUCTURE_USED_VARS_def,
                          IN_UNION, SUBSET_DEF, GSYM PATH_USED_VARS_THM] THEN
-        PROVE_TAC[]
+        PROVE_TAC []
       ]
     ]
-  );
+QED
 
+Theorem LTL_RECURSION_LAWS___LTL_ALWAYS :
+    !f. LTL_EQUIVALENT (LTL_ALWAYS f)
+                       (LTL_AND(f, LTL_NEXT(LTL_ALWAYS f)))
+Proof
+    REWRITE_TAC [LTL_EQUIVALENT_def, LTL_SEM_THM]
+ >> rpt STRIP_TAC
+ >> EQ_TAC >> rpt STRIP_TAC
+ >| [ `t >= t` by DECIDE_TAC >> PROVE_TAC [],
+      `k >= t` by DECIDE_TAC >> PROVE_TAC [],
+      Cases_on `k = t` >|
+      [ PROVE_TAC [],
+       `k >= SUC t` by DECIDE_TAC \\
+        PROVE_TAC [] ] ]
+QED
 
+Theorem LTL_RECURSION_LAWS___LTL_EVENTUAL :
+    !f. LTL_EQUIVALENT (LTL_EVENTUAL f)
+                       (LTL_OR(f, LTL_NEXT(LTL_EVENTUAL f)))
+Proof
+    REWRITE_TAC [LTL_EQUIVALENT_def, LTL_SEM_THM]
+ >> rpt STRIP_TAC
+ >> EQ_TAC >> rpt STRIP_TAC
+ >| [ Cases_on `k = t` >|
+      [ PROVE_TAC [],
+       `k >= SUC t` by DECIDE_TAC >> PROVE_TAC [] ],
+     `t >= t` by DECIDE_TAC >> PROVE_TAC [],
+     `k >= t` by DECIDE_TAC >> PROVE_TAC [] ]
+QED
 
-val LTL_RECURSION_LAWS___LTL_ALWAYS =
- store_thm
-  ("LTL_RECURSION_LAWS___LTL_ALWAYS",
-   ``!f. LTL_EQUIVALENT (LTL_ALWAYS f) (LTL_AND(f, LTL_NEXT(LTL_ALWAYS f)))``,
-
-   REWRITE_TAC [LTL_EQUIVALENT_def, LTL_SEM_THM] THEN
-   REPEAT STRIP_TAC THEN
-   EQ_TAC THEN REPEAT STRIP_TAC THENL [
-      `t >= t` by DECIDE_TAC THEN
-      PROVE_TAC[],
-
-      `k >= t` by DECIDE_TAC THEN
-      PROVE_TAC[],
-
-      Cases_on `k = t` THENL [
-         PROVE_TAC[],
-
-         `k >= SUC t` by DECIDE_TAC THEN
-         PROVE_TAC[]
-      ]
-   ]);
-
-
-val LTL_RECURSION_LAWS___LTL_EVENTUAL =
- store_thm
-  ("LTL_RECURSION_LAWS___LTL_EVENTUAL",
-   ``!f. LTL_EQUIVALENT (LTL_EVENTUAL f) (LTL_OR(f, LTL_NEXT(LTL_EVENTUAL f)))``,
-
-   REWRITE_TAC [LTL_EQUIVALENT_def, LTL_SEM_THM] THEN
-   REPEAT STRIP_TAC THEN
-   EQ_TAC THEN REPEAT STRIP_TAC THENL [
-      Cases_on `k = t` THENL [
-         PROVE_TAC[],
-
-         `k >= SUC t` by DECIDE_TAC THEN
-         PROVE_TAC[]
-      ],
-
-      `t >= t` by DECIDE_TAC THEN
-      PROVE_TAC[],
-
-      `k >= t` by DECIDE_TAC THEN
-      PROVE_TAC[]
-   ]);
-
-
-
-val LTL_RECURSION_LAWS___LTL_SUNTIL =
- store_thm
-  ("LTL_RECURSION_LAWS___LTL_SUNTIL",
-   ``!l1 l2. LTL_EQUIVALENT (LTL_SUNTIL (l1, l2))
-                            (LTL_OR(l2, LTL_AND(l1, LTL_NEXT(LTL_SUNTIL (l1, l2)))))``,
-
-
-SIMP_TAC std_ss [LTL_EQUIVALENT_def, LTL_SEM_THM] THEN
-REPEAT STRIP_TAC THEN EQ_TAC THEN REPEAT STRIP_TAC THENL [
+Theorem LTL_RECURSION_LAWS___LTL_SUNTIL :
+    !l1 l2. LTL_EQUIVALENT (LTL_SUNTIL (l1, l2))
+                           (LTL_OR(l2, LTL_AND(l1, LTL_NEXT(LTL_SUNTIL (l1, l2)))))
+Proof
+    SIMP_TAC std_ss [LTL_EQUIVALENT_def, LTL_SEM_THM]
+ >> rpt STRIP_TAC THEN EQ_TAC THEN rpt STRIP_TAC THENL [
   Cases_on `k = t` THENL [
     PROVE_TAC[],
 
     DISJ2_TAC THEN
-    REPEAT STRIP_TAC THENL [
+    rpt STRIP_TAC THENL [
       `t <= t /\ t < k` by DECIDE_TAC THEN
       PROVE_TAC[],
 
       EXISTS_TAC ``k:num`` THEN
-      REPEAT STRIP_TAC THENL [
+      rpt STRIP_TAC THENL [
         DECIDE_TAC,
         ASM_REWRITE_TAC[],
         `t <= j` by DECIDE_TAC THEN PROVE_TAC[]
@@ -938,42 +856,36 @@ REPEAT STRIP_TAC THEN EQ_TAC THEN REPEAT STRIP_TAC THENL [
     ]
   ],
 
-
   EXISTS_TAC ``t:num`` THEN
   ASM_SIMP_TAC arith_ss [],
 
-
   EXISTS_TAC ``k:num`` THEN
   ASM_SIMP_TAC arith_ss [] THEN
-  REPEAT STRIP_TAC THEN
+  rpt STRIP_TAC THEN
   Cases_on `j = t` THENL [
     PROVE_TAC[],
     `SUC t <= j` by DECIDE_TAC THEN PROVE_TAC[]
   ]
-]);
+]
+QED
 
-
-
-val LTL_RECURSION_LAWS___LTL_PSUNTIL =
- store_thm
-  ("LTL_RECURSION_LAWS___LTL_PSUNTIL",
-   ``!l1 l2. LTL_EQUIVALENT (LTL_PSUNTIL (l1, l2))
-                            (LTL_OR(l2, LTL_AND(l1, LTL_PSNEXT(LTL_PSUNTIL (l1, l2)))))``,
-
-
-SIMP_TAC std_ss [LTL_EQUIVALENT_def, LTL_SEM_THM] THEN
-REPEAT STRIP_TAC THEN EQ_TAC THEN REPEAT STRIP_TAC THENL [
+Theorem LTL_RECURSION_LAWS___LTL_PSUNTIL :
+    !l1 l2. LTL_EQUIVALENT (LTL_PSUNTIL (l1, l2))
+                           (LTL_OR(l2, LTL_AND(l1, LTL_PSNEXT(LTL_PSUNTIL (l1, l2)))))
+Proof
+    SIMP_TAC std_ss [LTL_EQUIVALENT_def, LTL_SEM_THM]
+ >> rpt STRIP_TAC THEN EQ_TAC THEN rpt STRIP_TAC THENL [
   Cases_on `k = t` THENL [
     PROVE_TAC[],
 
     DISJ2_TAC THEN
     Cases_on `t` THEN SIMP_ALL_TAC arith_ss [] THEN
-    REPEAT STRIP_TAC THENL [
+    rpt STRIP_TAC THENL [
       `SUC n <= SUC n /\ k < SUC n` by DECIDE_TAC THEN
       PROVE_TAC[],
 
       EXISTS_TAC ``k:num`` THEN
-      REPEAT STRIP_TAC THENL [
+      rpt STRIP_TAC THENL [
         DECIDE_TAC,
         ASM_REWRITE_TAC[],
         `j <= SUC n` by DECIDE_TAC THEN PROVE_TAC[]
@@ -981,42 +893,37 @@ REPEAT STRIP_TAC THEN EQ_TAC THEN REPEAT STRIP_TAC THENL [
     ]
   ],
 
-
   EXISTS_TAC ``t:num`` THEN
   ASM_SIMP_TAC arith_ss [],
 
-
   EXISTS_TAC ``k:num`` THEN
   ASM_SIMP_TAC arith_ss [] THEN
-  REPEAT STRIP_TAC THEN
+  rpt STRIP_TAC THEN
   Cases_on `j = t` THENL [
     PROVE_TAC[],
     `j <= PRE t` by DECIDE_TAC THEN PROVE_TAC[]
   ]
-]);
+]
+QED
 
+Theorem LTL_EVENTUAL___PALWAYS :
+    !k w p. LTL_SEM_TIME k w (LTL_EVENTUAL p) ==>
+            !l. l <= k ==> LTL_SEM_TIME l w (LTL_EVENTUAL p)
+Proof
+    REWRITE_TAC [LTL_SEM_THM]
+ >> rpt STRIP_TAC
+ >> EXISTS_TAC ``k':num``
+ >> ASM_REWRITE_TAC []
+ >> DECIDE_TAC
+QED
 
-val LTL_EVENTUAL___PALWAYS =
- store_thm
-  ("LTL_EVENTUAL___PALWAYS",
-   ``!k w p. (LTL_SEM_TIME k w (LTL_EVENTUAL p)) ==>
-      (!l. l <= k ==> LTL_SEM_TIME l w (LTL_EVENTUAL p))``,
-
-   REWRITE_TAC[LTL_SEM_THM] THEN
-   REPEAT STRIP_TAC THEN
-   EXISTS_TAC ``k':num`` THEN
-   ASM_REWRITE_TAC[] THEN
-   DECIDE_TAC);
-
-
-val LTL_WEAK_UNTIL___ALTERNATIVE_DEF =
- store_thm
-  ("LTL_WEAK_UNTIL___ALTERNATIVE_DEF",
-   ``!f1 f2. LTL_EQUIVALENT (LTL_UNTIL(f1,f2)) (LTL_NOT (LTL_SUNTIL(LTL_NOT f2, LTL_AND(LTL_NOT f1, LTL_NOT f2))))``,
-
-   SIMP_TAC std_ss [LTL_EQUIVALENT_def, LTL_UNTIL_def, LTL_SEM_THM] THEN
-   REPEAT STRIP_TAC THEN
-   EQ_TAC THEN REPEAT STRIP_TAC THENL [
+Theorem LTL_WEAK_UNTIL___ALTERNATIVE_DEF :
+    !f1 f2. LTL_EQUIVALENT (LTL_UNTIL(f1,f2))
+                           (LTL_NOT (LTL_SUNTIL(LTL_NOT f2, LTL_AND(LTL_NOT f1, LTL_NOT f2))))
+Proof
+    SIMP_TAC std_ss [LTL_EQUIVALENT_def, LTL_UNTIL_def, LTL_SEM_THM]
+ >> rpt STRIP_TAC
+ >> EQ_TAC THEN rpt STRIP_TAC THENL [
       Cases_on `k < k'` THENL [
          `t <= k` by DECIDE_TAC THEN
          METIS_TAC[],
@@ -1034,7 +941,8 @@ val LTL_WEAK_UNTIL___ALTERNATIVE_DEF =
 
          DISJ1_TAC THEN
          SIMP_ASSUMPTIONS_TAC std_ss [] THEN
-         SUBGOAL_TAC `?k. (k >= t /\ ~LTL_SEM_TIME k w f1) /\ !k'. k' < k ==> ~(k' >= t /\ ~LTL_SEM_TIME k' w f1)` THEN1 (
+         SUBGOAL_TAC `?k. (k >= t /\ ~LTL_SEM_TIME k w f1) /\
+                          !k'. k' < k ==> ~(k' >= t /\ ~LTL_SEM_TIME k' w f1)` THEN1 (
             ASSUME_TAC (EXISTS_LEAST_CONV ``?k. k >= t /\ ~LTL_SEM_TIME k w f1``) THEN
             RES_TAC THEN PROVE_TAC[]
          ) THEN
@@ -1050,22 +958,20 @@ val LTL_WEAK_UNTIL___ALTERNATIVE_DEF =
          ) THEN
          EXISTS_TAC ``l:num`` THEN
          ASM_SIMP_TAC arith_ss [] THEN
-         REPEAT STRIP_TAC THEN
+         rpt STRIP_TAC THEN
          `j < k' /\ j >= t` by DECIDE_TAC THEN
          METIS_TAC[]
       ]
-   ]);
+   ]
+QED
 
-
-
-val LTL_PAST_WEAK_UNTIL___ALTERNATIVE_DEF =
- store_thm
-  ("LTL_PAST_WEAK_UNTIL___ALTERNATIVE_DEF",
-   ``!f1 f2. LTL_EQUIVALENT (LTL_PUNTIL(f1,f2)) (LTL_NOT (LTL_PSUNTIL(LTL_NOT f2, LTL_AND(LTL_NOT f1, LTL_NOT f2))))``,
-
-   SIMP_TAC std_ss [LTL_EQUIVALENT_def, LTL_PUNTIL_def, LTL_SEM_THM] THEN
-   REPEAT STRIP_TAC THEN
-   EQ_TAC THEN REPEAT STRIP_TAC THENL [
+Theorem LTL_PAST_WEAK_UNTIL___ALTERNATIVE_DEF :
+    !f1 f2. LTL_EQUIVALENT (LTL_PUNTIL(f1,f2))
+                           (LTL_NOT (LTL_PSUNTIL(LTL_NOT f2, LTL_AND(LTL_NOT f1, LTL_NOT f2))))
+Proof
+    SIMP_TAC std_ss [LTL_EQUIVALENT_def, LTL_PUNTIL_def, LTL_SEM_THM]
+ >> rpt STRIP_TAC
+ >> EQ_TAC THEN rpt STRIP_TAC THENL [
       Cases_on `k' < k` THENL [
          `k' < k` by DECIDE_TAC THEN
          METIS_TAC[],
@@ -1083,7 +989,7 @@ val LTL_PAST_WEAK_UNTIL___ALTERNATIVE_DEF =
       `?P. P = \k. k <= t /\ ~(LTL_SEM_TIME k w f1)` by METIS_TAC[] THEN
       SUBGOAL_TAC `?x. P x /\ !z. z > x ==> ~(P z)` THEN1 (
         ASM_SIMP_TAC std_ss [GSYM arithmeticTheory.EXISTS_GREATEST] THEN
-        REPEAT STRIP_TAC THENL [
+        rpt STRIP_TAC THENL [
           METIS_TAC[],
 
           Q_TAC EXISTS_TAC `t` THEN
@@ -1092,7 +998,7 @@ val LTL_PAST_WEAK_UNTIL___ALTERNATIVE_DEF =
       ) THEN
       NTAC 2 (UNDISCH_HD_TAC) THEN
       ASM_SIMP_TAC std_ss [] THEN
-      REPEAT STRIP_TAC THEN
+      rpt STRIP_TAC THEN
       SUBGOAL_TAC `?x'. (x' >= x)  /\ (x' <= t) /\ LTL_SEM_TIME x' w f2` THEN1 (
         Q_SPEC_NO_ASSUM 6 `x` THEN
         CLEAN_ASSUMPTIONS_TAC THENL [
@@ -1105,34 +1011,31 @@ val LTL_PAST_WEAK_UNTIL___ALTERNATIVE_DEF =
       ) THEN
       Q_TAC EXISTS_TAC `x'` THEN
       ASM_SIMP_TAC arith_ss [] THEN
-      REPEAT STRIP_TAC THEN
+      rpt STRIP_TAC THEN
       `j > x` by DECIDE_TAC THEN
       METIS_TAC[]
-  ]);
+  ]
+QED
 
+Theorem LTL_STRONG___WEAK__IMPL___UNTIL :
+    !k w p1 p2. LTL_SEM_TIME k w (LTL_SUNTIL(p1, p2)) ==>
+                LTL_SEM_TIME k w (LTL_UNTIL(p1, p2))
+Proof
+    REWRITE_TAC [LTL_UNTIL_def, LTL_OR_SEM]
+ >> PROVE_TAC []
+QED
 
-
-val LTL_STRONG___WEAK__IMPL___UNTIL =
- store_thm
-  ("LTL_STRONG___WEAK__IMPL___UNTIL",
-   ``!k w p1 p2.
-      ((LTL_SEM_TIME k w (LTL_SUNTIL(p1, p2))) ==> (LTL_SEM_TIME k w (LTL_UNTIL(p1, p2))))``,
-
-   REWRITE_TAC[LTL_UNTIL_def, LTL_OR_SEM] THEN
-   PROVE_TAC[]);
-
-val LTL_COND___OR =
- store_thm
-  ("LTL_COND___OR",
-   ``!k w c p1 p2. (LTL_SEM_TIME k w (LTL_COND (c, p1, p2))) ==>
-                    (LTL_SEM_TIME k w (LTL_OR (p1, p2)))``,
-
-   REWRITE_TAC[LTL_SEM_THM, LTL_COND_def] THEN
-   METIS_TAC[]);
+Theorem LTL_COND___OR :
+    !k w c p1 p2. LTL_SEM_TIME k w (LTL_COND (c, p1, p2)) ==>
+                  LTL_SEM_TIME k w (LTL_OR (p1, p2))
+Proof
+    REWRITE_TAC [LTL_SEM_THM, LTL_COND_def]
+ >> METIS_TAC []
+QED
 
 Theorem LTL_MONOTICITY_LAWS :
-    !As Aw Bs Bw v. ((!t. LTL_SEM_TIME t v Aw ==> LTL_SEM_TIME t v As) /\
-                     (!t. LTL_SEM_TIME t v Bw ==> LTL_SEM_TIME t v Bs)) ==>
+    !As Aw Bs Bw v. (!t. LTL_SEM_TIME t v Aw ==> LTL_SEM_TIME t v As) /\
+                    (!t. LTL_SEM_TIME t v Bw ==> LTL_SEM_TIME t v Bs) ==>
          (!t. LTL_SEM_TIME t v (LTL_NOT As) ==> LTL_SEM_TIME t v (LTL_NOT Aw)) /\
          (!t. LTL_SEM_TIME t v (LTL_NEXT Aw) ==> LTL_SEM_TIME t v (LTL_NEXT As)) /\
          (!t. LTL_SEM_TIME t v (LTL_AND(Aw, Bw)) ==> LTL_SEM_TIME t v (LTL_AND(As, Bs))) /\
